Program level completed

SIMP/ARINC653_MultiCore_Que.thy
@@ -1,8 +1,9 @@
 theory ARINC653_MultiCore_Que
-  imports PiCore_SIMP_Syntax "../PiCore_RG_IFS"
+  imports PiCore_SIMP_Syntax Ref_SIMP PiCore_SIMP_Ref
 begin
 
-subsection \<open>functional specification\<close>
+
+subsection \<open>System specification\<close>
 
 type_synonym max_buffer_size = nat
 type_synonym buffer_size = nat
@@ -21,15 +22,9 @@ record Config = c2s :: "Core \<Rightarrow> Sched"
                 chsrc :: "QChannel \<Rightarrow> Port"
                 chdest :: "QChannel \<Rightarrow> Port"  
                 chmax :: "QChannel \<Rightarrow> nat"
-  
 axiomatization conf::Config 
   where bij_c2s: "bij (c2s conf)" 
-(*
-    and surj_p2c: "surj (p2s conf)" 
-    and portsrc_disj: "\<forall>c1 c2. c1 \<noteq> c2 \<longrightarrow> (chsrc conf) c1 \<noteq> (chsrc conf) c2" 
-    and portdest_disj: "\<forall>c1 c2. c1 \<noteq> c2 \<longrightarrow> (chdest conf) c1 \<noteq> (chdest conf) c2" 
-*)
-
+  
 lemma inj_surj_c2s: "inj (c2s conf) \<and> surj (c2s conf)"
   using bij_c2s by (simp add: bij_def) 
 
@@ -50,561 +45,22 @@ definition ch_destqport :: "Config \<Rightarrow> Port \<Rightarrow> QChannel"
 
 datatype PartMode = IDLE | READY | RUN
 
-record State = cur :: "Sched \<Rightarrow> Part option"
-               qlock :: "QChannel \<Rightarrow> Core option"
-               qbuf :: "QChannel \<Rightarrow> Message list"
-               qbufsize :: "QChannel \<Rightarrow> nat"
-               rflag :: "Core \<Rightarrow> bool"
-               partst :: "Part \<Rightarrow> PartMode"
-
 datatype EL = Core_InitE | ScheduleE | Send_Que_MessageE |  Recv_Que_MessageE
 
 datatype parameter = Port Port | Message Message | Partition Part
 
+datatype Domain = P Part | S Sched | F 
+
 type_synonym EventLabel = "EL \<times> (parameter list \<times> Core)" 
-type_synonym Prog = "State com option"
 
 definition get_evt_label :: "EL \<Rightarrow> parameter list \<Rightarrow> Core \<Rightarrow> EventLabel" ("_ _ \<rhd> _" [0,0,0] 20)
   where "get_evt_label el ps k \<equiv> (el,(ps,k))"
 
-definition get_evt_core :: "(EventLabel, Core, State, Prog) event \<Rightarrow> Core"
+definition get_evt_core :: "(EventLabel, 'k , 's, 'prog) event \<Rightarrow> Core"
   where "get_evt_core ev =  snd (snd (the (label_e ev)))"
 
-definition get_evt_el :: "(EventLabel, Core, State, Prog) event \<Rightarrow> EL"
+definition get_evt_el :: "(EventLabel, 'k , 's, 'prog) event \<Rightarrow> EL"
   where "get_evt_el ev =  fst (the (label_e ev))"
-
-definition Core_Init :: "Core \<Rightarrow> (EventLabel, Core, State, Prog) event" 
-  where "Core_Init k \<equiv> 
-    EVENT Core_InitE [] \<rhd> k 
-    THEN      
-      (\<acute>partst := (\<lambda>p. if p2s conf p = c2s conf k \<and> \<acute>partst p = IDLE then READY else \<acute>partst p)) 
-    END"
-
-definition System_Init :: "Config \<Rightarrow> (State \<times> (EventLabel, Core, State, Prog) x)"
-  where "System_Init cfg \<equiv> (\<lparr>cur=(\<lambda>s. None),
-                            qlock = (\<lambda>c. None),
-                            qbuf = (\<lambda>c. []),
-                            qbufsize = (\<lambda>c. 0),
-                            rflag = (\<lambda>C. False),
-                            partst = (\<lambda>p. IDLE)\<rparr>, 
-                            (\<lambda>k. Core_Init k))"
-
-definition Schedule :: "Core \<Rightarrow> Part \<Rightarrow> (EventLabel, Core, State, Prog) event" 
-  where "Schedule k p \<equiv> 
-    EVENT ScheduleE [Partition p] \<rhd> k 
-    WHERE
-      p2s conf p = c2s conf k \<and> (\<acute>partst p \<noteq> IDLE) \<and> (\<acute>cur (c2s conf k) = None 
-          \<or> p2s conf (the (\<acute>cur((c2s conf) k))) = c2s conf k)
-    THEN
-        IF (\<acute>cur((c2s conf) k) \<noteq> None) THEN    
-              ATOMIC
-           \<acute>partst := \<acute>partst(the (\<acute>cur ((c2s conf) k)) := READY);;
-           \<acute>cur := \<acute>cur((c2s conf) k := None)
-               END
-            FI;;  
-
-      (ATOMIC
-         \<acute>cur := \<acute>cur((c2s conf k) := Some p);;
-         \<acute>partst := \<acute>partst(p := RUN)
-        END)
-    END"
-
-definition Send_Que_Message :: "Core \<Rightarrow> Port \<Rightarrow> Message \<Rightarrow> (EventLabel, Core, State, Prog) event" 
-  where "Send_Que_Message k p m \<equiv> 
-    EVENT Send_Que_MessageE [Port p, Message m] \<rhd> k 
-    WHERE
-      is_src_qport conf p
-      \<and> \<acute>cur (c2s conf k) \<noteq> None
-      \<and> port_of_part conf p (the (\<acute>cur (c2s conf k)))
-    THEN
-      AWAIT \<acute>qlock (ch_destqport conf p) = None THEN
-        \<acute>qlock := \<acute>qlock (ch_destqport conf p := Some k) 
-      END;;
-      IF \<acute>qbufsize (ch_srcqport conf p) < chmax conf (ch_srcqport conf p) THEN 
-        \<acute>qbuf := \<acute>qbuf (ch_srcqport conf p := \<acute>qbuf (ch_srcqport conf p) @ [m]);;
-        \<acute>qbufsize := \<acute>qbufsize (ch_srcqport conf p := \<acute>qbufsize (ch_srcqport conf p) + 1)
-      FI;;
-      \<acute>qlock := \<acute>qlock (ch_destqport conf p := None)
-    END"
-
-definition Recv_Que_Message :: "Core \<Rightarrow> Port \<Rightarrow> (EventLabel, Core, State, Prog) event" 
-  where "Recv_Que_Message k p \<equiv> 
-    EVENT Recv_Que_MessageE [Port p] \<rhd> k 
-    WHERE
-      is_dest_qport conf p 
-      \<and> \<acute>cur (c2s conf k) \<noteq> None
-      \<and> port_of_part conf p (the (\<acute>cur (c2s conf k)))
-    THEN 
-    \<acute>rflag := \<acute>rflag (k := False);;
-    WHILE \<not> (\<acute>rflag k) DO
-      AWAIT \<acute>qlock (ch_destqport conf p) = None THEN
-        \<acute>qlock := \<acute>qlock (ch_destqport conf p := Some k)
-      END;;
-      IF \<acute>qbufsize (ch_srcqport conf p) > 0 THEN 
-        \<acute>qbuf := \<acute>qbuf (ch_destqport conf p := tl (\<acute>qbuf (ch_destqport conf p)));;
-        \<acute>qbufsize := \<acute>qbufsize (ch_destqport conf p := \<acute>qbufsize (ch_destqport conf p) - 1);;
-        \<acute>rflag := \<acute>rflag (k := True)
-      FI;;
-      \<acute>qlock := \<acute>qlock (ch_destqport conf p := None)
-      OD
-    END"
-
-subsection \<open>Rely-guarantee condition of events\<close>
-
-abbreviation "core_init_pre k \<equiv> \<lbrace>\<forall>p. p2s conf p = c2s conf k \<longrightarrow> \<acute>partst p = IDLE\<rbrace>"
-abbreviation "core_init_rely k \<equiv> \<lbrace>(\<forall>p. p2s conf p = c2s conf k \<longrightarrow> \<ordfeminine>partst p = \<ordmasculine>partst p)\<rbrace>"
-abbreviation "core_init_guar k \<equiv> \<lbrace>\<ordfeminine>cur= \<ordmasculine>cur \<and> \<ordfeminine>qbuf= \<ordmasculine>qbuf \<and> \<ordfeminine>qbufsize= \<ordmasculine>qbufsize 
-            \<and> (\<forall>p. p2s conf p = c2s conf k \<longrightarrow> \<ordmasculine>partst p = IDLE \<and> \<ordfeminine>partst p = READY)
-            \<and> (\<forall>c p. c \<noteq> k \<and> p2s conf p = c2s conf c \<longrightarrow> \<ordfeminine>partst  p = \<ordmasculine>partst p)\<rbrace> \<union> Id"
-abbreviation "core_init_post \<equiv> \<lbrace>True\<rbrace>"
-
-definition Core_Init_RGCond :: " Core \<Rightarrow> (State) rgformula"
-  where "Core_Init_RGCond  k \<equiv> RG[core_init_pre k, core_init_rely k, core_init_guar k, core_init_post]"
-
-abbreviation "schedule_pre \<equiv> \<lbrace>True\<rbrace>"
-abbreviation "schedule_rely k \<equiv> \<lbrace>\<ordfeminine>cur (c2s conf k) = \<ordmasculine>cur  (c2s conf k) \<and>
-              (\<forall>p. p2s conf p = c2s conf k \<longrightarrow> \<ordfeminine>partst  p = \<ordmasculine>partst p)\<rbrace>"
-
-abbreviation "schedule_guar k p \<equiv> 
-  \<lbrace>(\<ordfeminine>cur = \<ordmasculine>cur(c2s conf k := Some p) \<and> \<ordfeminine>partst = \<ordmasculine>partst(the (\<ordfeminine>cur(c2s conf k)) := RUN) 
-   \<and> p2s conf p = c2s conf k \<or> (\<ordfeminine>cur = \<ordmasculine>cur(c2s conf k := None) 
-   \<and> \<ordfeminine>partst = \<ordmasculine>partst(the (\<ordmasculine>cur (c2s conf k)) := READY)))
-   \<and> (\<forall>c. c \<noteq> k \<longrightarrow> \<ordfeminine>cur (c2s conf c) = \<ordmasculine>cur  (c2s conf c))
-   \<and> (\<forall>p. p2s conf p \<noteq> c2s conf k \<longrightarrow> \<ordfeminine>partst  p = \<ordmasculine>partst p )
-   \<and> \<ordfeminine>qbuf= \<ordmasculine>qbuf  \<and> \<ordfeminine>qbufsize= \<ordmasculine>qbufsize\<rbrace> \<union> Id"
-
-abbreviation "schedule_post \<equiv> \<lbrace>True\<rbrace>"
-
-definition Schedule_RGCond :: "Core \<Rightarrow> Part \<Rightarrow>(State) rgformula"
-  where "Schedule_RGCond k p \<equiv> RG[schedule_pre, schedule_rely k, schedule_guar k p, schedule_post]"
-
-abbreviation "snd_recv_pre \<equiv> \<lbrace>True\<rbrace>"
-abbreviation "snd_recv_rely k \<equiv> \<lbrace>\<ordfeminine>cur (c2s conf k) = \<ordmasculine>cur  (c2s conf k)\<rbrace>"
-abbreviation "snd_send_guar k p \<equiv> 
-    \<lbrace>\<ordfeminine>cur = \<ordmasculine>cur \<and> \<ordfeminine>partst = \<ordmasculine>partst \<and> (\<ordmasculine>qbufsize (ch_srcqport conf p) = length (\<ordmasculine>qbuf (ch_srcqport conf p))
-      \<longrightarrow> \<ordfeminine>qbufsize (ch_srcqport conf p) = length (\<ordfeminine>qbuf (ch_srcqport conf p))) \<and>
-    ((is_src_qport conf p \<and> \<ordmasculine>cur (c2s conf k) \<noteq> None \<and> port_of_part conf p (the (\<ordmasculine>cur (c2s conf k)))) \<longrightarrow>
-    (\<forall>c. c \<noteq> ch_srcqport conf p \<longrightarrow> \<ordfeminine>qbuf c = \<ordmasculine>qbuf c \<and> \<ordfeminine>qbufsize c = \<ordmasculine>qbufsize c)) \<and> 
-    ((\<not>(is_src_qport conf p \<and> \<ordmasculine>cur ((c2s conf) k) \<noteq> None \<and> port_of_part conf p (the (\<ordmasculine>cur ((c2s conf) k)))))
-    \<longrightarrow> (\<ordfeminine>qbuf  = \<ordmasculine>qbuf  \<and> \<ordfeminine>qbufsize  = \<ordmasculine>qbufsize))\<rbrace>"
-
-
-abbreviation "snd_recv_guar k p \<equiv> 
-    \<lbrace>\<ordfeminine>cur = \<ordmasculine>cur \<and> \<ordfeminine>partst = \<ordmasculine>partst \<and>  (\<ordmasculine>qbufsize (ch_destqport conf p) = length (\<ordmasculine>qbuf (ch_destqport conf p))
-      \<longrightarrow> \<ordfeminine>qbufsize (ch_destqport conf p) = length (\<ordfeminine>qbuf (ch_destqport conf p))) \<and>
-    ((is_dest_qport conf p \<and> \<ordmasculine>cur ((c2s conf) k) \<noteq> None \<and> port_of_part conf p (the (\<ordmasculine>cur ((c2s conf) k)))) \<longrightarrow>
-    (\<forall>c. c \<noteq> ch_destqport conf p \<longrightarrow> \<ordfeminine>qbuf c = \<ordmasculine>qbuf c \<and> \<ordfeminine>qbufsize c = \<ordmasculine>qbufsize c)) \<and> 
-    ((\<not>(is_dest_qport conf p \<and> \<ordmasculine>cur ((c2s conf) k) \<noteq> None \<and> port_of_part conf p (the (\<ordmasculine>cur ((c2s conf) k)))))
-    \<longrightarrow> (\<ordfeminine>qbuf  = \<ordmasculine>qbuf  \<and> \<ordfeminine>qbufsize  = \<ordmasculine>qbufsize))\<rbrace>"
-
-abbreviation "snd_recv_post \<equiv> \<lbrace>True\<rbrace>"
-
-definition Send_Que_Message_RGCond :: "Core \<Rightarrow> Port \<Rightarrow> Message \<Rightarrow> (State) rgformula"
-  where "Send_Que_Message_RGCond k p m \<equiv> RG[snd_recv_pre, snd_recv_rely k, snd_send_guar k p, snd_recv_post]"
-
-definition Recv_Que_Message_RGCond :: "Core \<Rightarrow> Port \<Rightarrow> (State) rgformula"
-  where "Recv_Que_Message_RGCond k p \<equiv> RG[snd_recv_pre, snd_recv_rely k, snd_recv_guar k p, snd_recv_post]"
-
-definition Core_Init_RGF :: "Core \<Rightarrow> (EventLabel, Core, State, Prog) rgformula_e"
-  where "Core_Init_RGF k \<equiv> (Core_Init k, Core_Init_RGCond k)"
-
-definition Schedule_RGF :: "Core \<Rightarrow> Part \<Rightarrow> (EventLabel, Core, State, Prog) rgformula_e"
-  where "Schedule_RGF k p \<equiv> (Schedule k p, Schedule_RGCond k p)"
-
-definition Send_Que_Message_RGF :: "Core \<Rightarrow> Port \<Rightarrow> Message \<Rightarrow> (EventLabel, Core, State, Prog) rgformula_e"
-  where "Send_Que_Message_RGF k p m \<equiv> (Send_Que_Message k p m, Send_Que_Message_RGCond k p m)"
-
-definition Recv_Que_Message_RGF :: "Core \<Rightarrow> Port \<Rightarrow> (EventLabel, Core, State, Prog) rgformula_e"
-  where "Recv_Que_Message_RGF k p  \<equiv> (Recv_Que_Message k p, Recv_Que_Message_RGCond k p)"
-
-definition EvtSys1_on_Core_RGF :: "Core \<Rightarrow> (EventLabel, Core, State, Prog) rgformula_es"
-  where "EvtSys1_on_Core_RGF k \<equiv> 
-            (rgf_EvtSys (\<Union>p.{Schedule_RGF k p} \<union>
-                          (\<Union>(p, m). {Send_Que_Message_RGF k p m}) \<union>
-                          (\<Union>p.{Recv_Que_Message_RGF k p})),
-               RG[\<lbrace>True\<rbrace>,\<lbrace>\<ordfeminine>cur (c2s conf k) = \<ordmasculine>cur  (c2s conf k) \<and> 
-                  (\<forall>p. p2s conf p = c2s conf k \<longrightarrow> \<ordfeminine>partst  p = \<ordmasculine>partst p)\<rbrace>,
-                  ((\<Union>p. schedule_guar k p) \<union> (\<Union>p. snd_send_guar k p) \<union> 
-                  (\<Union>p. snd_recv_guar k p) \<union> Id), \<lbrace>True\<rbrace>])"
-
-definition EvtSys_on_Core_RGF :: "Core \<Rightarrow> (EventLabel, Core, State, Prog) rgformula_es"
-  where "EvtSys_on_Core_RGF k  \<equiv> 
-          (rgf_EvtSeq (Core_Init_RGF k) (EvtSys1_on_Core_RGF k),
-           RG[core_init_pre k,
-              schedule_rely k,
-              ((\<Union>p. schedule_guar k p) \<union> (\<Union>p. snd_send_guar k p) \<union> 
-              (\<Union>p. snd_recv_guar k p) \<union> Id \<union> (core_init_guar k)), \<lbrace>True\<rbrace>])"
-
-definition ARINCXKernel_Spec :: "(EventLabel, Core, State, Prog) rgformula_par"
-  where "ARINCXKernel_Spec \<equiv> (\<lambda>k. EvtSys_on_Core_RGF k)"
-                                       
-
-axiomatization s0 where s0_init: "s0 \<equiv> fst (System_Init conf)"
-axiomatization x0 where x0_init: "x0 \<equiv> snd (System_Init conf)"
-axiomatization C0 where C0_init: "C0 = (paresys_spec ARINCXKernel_Spec, s0, x0)"
-
-subsection \<open>Functional correctness by rely guarantee proof\<close>
-
-definition Evt_sat_RG:: "'Env \<Rightarrow> (EventLabel, Core, State, Prog) event \<Rightarrow> (State) rgformula \<Rightarrow> bool" ("(_\<turnstile>_ sat _)" [60, 60,60] 61)
-  where "Evt_sat_RG \<Gamma> e rg \<equiv>  \<Gamma> \<turnstile> e sat\<^sub>e [Pre\<^sub>f rg, Rely\<^sub>f rg, Guar\<^sub>f rg, Post\<^sub>f rg]"
-
-
-lemma Core_Init_SatRG: "\<forall>k. \<Gamma> \<turnstile> (Core_Init k) sat Core_Init_RGCond k"
-  apply(simp add:Evt_sat_RG_def)
-  apply(rule allI)
-  apply(simp add:Core_Init_def)
-  apply(rule BasicEvt)
-    apply(simp add:body_def Core_Init_RGCond_def Pre\<^sub>f_def Post\<^sub>f_def  Rely\<^sub>f_def Guar\<^sub>f_def getrgformula_def)
-    apply(rule Basic, simp, simp)
-      apply auto
-  using inj_surj_c2s injI surj_def apply (simp add: inj_eq)
-     apply(simp add:stable_def)+
-     apply(simp add:guard_def stable_def)
-    apply (simp add: stable_def)
-   apply(simp add:Core_Init_RGCond_def Pre\<^sub>f_def Rely\<^sub>f_def getrgformula_def stable_def stable_e_def)
-  apply(simp add:Core_Init_RGCond_def Pre\<^sub>f_def Guar\<^sub>f_def  getrgformula_def stable_def)
-  done
-
-
-lemma Sched_SatRG_h1:
-    " \<turnstile>\<^sub>I Some (\<lbrace>True \<rbrace>\<acute>partst := \<acute>partst(the (\<acute>cur (c2s conf k)) := READY);;
-       \<lbrace>True \<rbrace> \<acute>cur := \<acute>cur (c2s conf k := None)) sat\<^sub>p 
-       [\<lbrace>p2s conf p = c2s conf k \<and> \<acute>partst p \<noteq> IDLE \<and> (\<acute>cur (c2s conf k) = None 
-        \<or> p2s conf (the (\<acute>cur (c2s conf k))) = c2s conf k)\<rbrace> \<inter> \<lbrace>\<exists>y. \<acute>cur (c2s conf k) = Some y\<rbrace> \<inter> {V}, 
-        {(s, t).s = t}, UNIV, 
-        \<lbrace>(\<acute>cur = (cur V)(c2s conf k \<mapsto> p) \<and> \<acute>partst = (partst V)(the (\<acute>cur (c2s conf k)) := RUN) \<and> 
-        p2s conf p = c2s conf k \<or> \<acute>cur = (cur V)(c2s conf k := None) \<and> \<acute>partst = (partst V)(the (cur V (c2s conf k)) := READY)) \<and>
-        (\<forall>c. c \<noteq> k \<longrightarrow> \<acute>cur (c2s conf c) = cur V (c2s conf c)) \<and> (\<forall>p. p2s conf p \<noteq> c2s conf k 
-        \<longrightarrow> \<acute>partst p = partst V p) \<and> \<acute>qbuf = qbuf V \<and> \<acute>qbufsize = qbufsize V \<or>\<acute>((=) V)\<rbrace> \<inter>
-        \<lbrace>p2s conf p = c2s conf k \<and> \<acute>cur (c2s conf k) = None\<rbrace>]"
-  apply(case_tac "p2s conf p = c2s conf k \<and> partst V p \<noteq> IDLE \<and> ((cur V) (c2s conf k) = None
-        \<or> p2s conf (the ((cur V) (c2s conf k))) = c2s conf k) \<and> (\<exists>y. (cur V) (c2s conf k) = Some y)")
-   apply simp
-   apply(rule Seq[where mid="{s. s = V \<lparr> partst := (partst V) (the ((cur V) (c2s conf k)) := READY)\<rparr>
-                              \<and> p2s conf p = c2s conf k}"])
-    apply simp
-    apply (rule Basic, simp)
-       apply auto[1]
-      apply(simp add:stable_def)+
-   apply (rule Basic, simp, simp)
-      apply(rule disjI1)
-      apply (rule conjI)
-  using inj_surj_c2s injI surj_def apply (simp add: inj_eq)
-      apply (rule impI)
-     apply(case_tac "cur V (c2s conf k) = None", simp)
-  using inj_surj_c2s injI surj_def apply (simp add: inj_eq)
-     apply simp
-    apply (simp add: stable_def)
-   apply (simp add: stable_def, clarify)
-   apply (intro conjI)
-       apply auto[1]
-      apply blast
-     apply blast
-    apply blast
-   apply blast
-  apply(rule Seq[where mid="{}"])
-   apply (rule Basic)
-       apply (simp add: stable_def)+
-  apply (rule Basic)
-      apply (simp add: stable_def)+
-  apply auto[1]
-  done
-
-lemma Sched_SatRG_h2: "\<turnstile>\<^sub>I Some (\<lbrace>True \<rbrace> \<acute>cur := \<acute>cur(c2s conf k \<mapsto> p) ;;
-                         \<lbrace>True \<rbrace> \<acute>partst := \<acute>partst (p := RUN))
-      sat\<^sub>p [\<lbrace>p2s conf p = c2s conf k \<and> \<acute>cur (c2s conf k) = None\<rbrace> \<inter> {V},  {(s, t). s = t}, UNIV, 
-           \<lbrace>(\<acute>cur = (cur V)(c2s conf k \<mapsto> p) \<and> \<acute>partst = (partst V)(the (\<acute>cur (c2s conf k)) := RUN) 
-           \<and> p2s conf p = c2s conf k \<or> \<acute>cur = (cur V)(c2s conf k := None) \<and> 
-             \<acute>partst = (partst V)(the (cur V (c2s conf k)) := READY)) \<and> 
-              (\<forall>c. c \<noteq> k \<longrightarrow> \<acute>cur (c2s conf c) = cur V (c2s conf c)) \<and> 
-              (\<forall>p. p2s conf p \<noteq> c2s conf k \<longrightarrow> \<acute>partst p = partst V p) \<and> \<acute>qbuf = qbuf V 
-              \<and> \<acute>qbufsize = qbufsize V \<or> \<acute>((=) V)\<rbrace>]"
-  apply(case_tac "p2s conf p = c2s conf k \<and> (cur V) (c2s conf k) = None", simp)
-   apply(rule Seq[where mid="{s. s = V \<lparr> cur := (cur V) (c2s conf k := Some p)\<rparr>}"])
-    apply (rule Basic)
-        apply (simp add: stable_def)+
-   apply (rule Basic, simp, simp)
-  using inj_surj_c2s injI surj_def apply (simp add: inj_eq)
-     apply(simp add:stable_def)+
-  apply(rule Seq[where mid="{}"])
-   apply (rule Basic, simp)
-      apply(simp add:stable_def)+
-  apply (rule Basic, simp)
-     apply (simp add: stable_def)+
-  done
-
-lemma Sched_SatRG: " \<Gamma> \<turnstile> (Schedule k p) sat Schedule_RGCond k p"
-  apply(simp add:Evt_sat_RG_def) 
-  apply(simp add:Schedule_def)
-  apply(rule BasicEvt) 
-    apply(simp add:body_def Schedule_RGCond_def guard_def Pre\<^sub>f_def  Post\<^sub>f_def Rely\<^sub>f_def Guar\<^sub>f_def getrgformula_def)
-    apply(rule Seq[where mid="\<lbrace>p2s conf p = c2s conf k \<and> \<acute>cur(c2s conf k) = None\<rbrace>"])
-     apply(rule Cond, simp)
-        apply(simp add: stable_def)
-       apply(rule Await)
-          apply force
-         apply(simp add: stable_def)+
-  using Sched_SatRG_h1 apply auto[1]
-      apply (rule Basic)
-          apply auto[1]
-         apply auto[1]
-        apply (clarsimp)
-       apply (simp add: stable_def)+
-    apply (rule Await, simp)
-      apply (simp add: stable_def)+
-    apply (rule allI)
-  using Sched_SatRG_h2 apply auto[1]
-   apply(simp add: stable_def Schedule_RGCond_def Pre\<^sub>f_def  Post\<^sub>f_def Guar\<^sub>f_def getrgformula_def stable_e_def)
-  apply(simp add: Schedule_RGCond_def Pre\<^sub>f_def Post\<^sub>f_def Guar\<^sub>f_def getrgformula_def)
-  done
-
-lemma Send_Que_Message_SatRG_h1: "\<turnstile>\<^sub>I Some (\<lbrace>True \<rbrace> \<acute>qbuf := \<acute>qbuf(ch_srcqport conf p := \<acute>qbuf (ch_srcqport conf p) @ [m]) ;;
-                                    \<lbrace>True \<rbrace> \<acute>qbufsize := \<acute>qbufsize (ch_srcqport conf p := Suc (\<acute>qbufsize (ch_srcqport conf p))))
-                sat\<^sub>p [\<lbrace>is_src_qport conf p \<and> (\<exists>y. \<acute>cur (c2s conf k) = Some y) \<and> 
-                      port_of_part conf p (the (\<acute>cur (c2s conf k)))\<rbrace> \<inter> {V} \<inter>
-                      \<lbrace>\<acute>qbufsize (ch_srcqport conf p) < chmax conf (ch_srcqport conf p)\<rbrace>, 
-                      {(s, t). s = t}, UNIV, \<lbrace>\<acute>cur = cur V \<and> \<acute>partst = partst V \<and> 
-                      (qbufsize V (ch_srcqport conf p) = length (qbuf V (ch_srcqport conf p)) \<longrightarrow> 
-                      \<acute>qbufsize (ch_srcqport conf p) = length (\<acute>qbuf (ch_srcqport conf p))) \<and>
-                       (is_src_qport conf p \<and> (\<exists>y. cur V (c2s conf k) = Some y) \<and> 
-                       port_of_part conf p (the (cur V (c2s conf k))) \<longrightarrow> (\<forall>c. c \<noteq> ch_srcqport conf p 
-                       \<longrightarrow> \<acute>qbuf c = qbuf V c \<and> \<acute>qbufsize c = qbufsize V c)) \<and> ((is_src_qport conf p 
-                      \<longrightarrow> cur V (c2s conf k) = None \<or> \<not> port_of_part conf p (the (cur V (c2s conf k)))) 
-                      \<longrightarrow> \<acute>qbuf = qbuf V \<and> \<acute>qbufsize = qbufsize V)\<rbrace>]"
-  apply(case_tac "is_src_qport conf p \<and> (\<exists>y. (cur V) ((c2s conf) k) = Some y) 
-       \<and> port_of_part conf p (the ((cur V) ((c2s conf) k))) 
-      \<and> (qbufsize V) (ch_srcqport conf p) < chmax conf (ch_srcqport conf p)")
-   apply simp
-   apply(rule Seq[where mid="{s. s = V\<lparr>qbuf := (qbuf V)(ch_srcqport conf p := (qbuf V) (ch_srcqport conf p) @ [m])\<rparr>}"])
-    apply(rule Basic)
-        apply auto[1]
-       apply(simp add: stable_def)+
-   apply(rule Basic, simp)
-       apply auto[1]
-      apply(simp add: stable_def)+
-  apply(rule Seq[where mid="{}"])
-   apply(rule Basic, simp)
-      apply(simp add:stable_def)+
-      apply fastforce
-     apply simp
-    apply (simp add: stable_def)+
-  apply(rule Basic)
-      apply(simp add:stable_def)+
-  done
-
-lemma Send_Que_Message_SatRG: 
-  " \<Gamma> \<turnstile> Send_Que_Message k p m sat Send_Que_Message_RGCond k p m"
-  apply(simp add:Evt_sat_RG_def)
-  apply(simp add:Send_Que_Message_def)
-  apply(rule BasicEvt)
-    apply(simp add:body_def Send_Que_Message_RGCond_def guard_def Pre\<^sub>f_def Post\<^sub>f_def Rely\<^sub>f_def 
-         Guar\<^sub>f_def getrgformula_def)
-    apply(rule Await)
-       apply(simp add: stable_def)+
-    apply(rule allI)
-    apply (rule Cond, simp)
-       apply (simp add: stable_def)
-  using Send_Que_Message_SatRG_h1 apply auto[1]
-     apply (rule Basic)
-         apply blast
-        apply force
-       apply simp
-      apply (simp add: stable_def)+
-   apply(simp add: stable_def Send_Que_Message_RGCond_def Pre\<^sub>f_def Rely\<^sub>f_def getrgformula_def stable_e_def)
-  apply(simp add: Send_Que_Message_RGCond_def Guar\<^sub>f_def getrgformula_def)
-  done
-
-lemma Recv_Que_Message_SatRG_h1: "\<turnstile>\<^sub>I Some (\<lbrace>True\<rbrace> \<acute>qbuf := \<acute>qbuf(ch_destqport conf p := tl (\<acute>qbuf (ch_destqport conf p)));;
-                         \<lbrace>True \<rbrace>\<acute>qbufsize := \<acute>qbufsize (ch_destqport conf p := \<acute>qbufsize (ch_destqport conf p) - Suc 0))
-            sat\<^sub>p [\<lbrace>is_dest_qport conf p \<and> (\<exists>y. \<acute>cur (c2s conf k) = Some y) \<and> port_of_part conf p (the (\<acute>cur (c2s conf k)))\<rbrace> 
-            \<inter> \<lbrace>0 < \<acute>qbufsize (ch_destqport conf p)\<rbrace> \<inter> {V}, {(s, t). s = t}, UNIV, 
-            \<lbrace>\<acute>cur = cur V \<and> \<acute>partst = partst V \<and> (qbufsize V (ch_destqport conf p) = length (qbuf V (ch_destqport conf p)) 
-            \<longrightarrow> \<acute>qbufsize (ch_destqport conf p) = length (\<acute>qbuf (ch_destqport conf p))) \<and>
-            (is_dest_qport conf p \<and> (\<exists>y. cur V (c2s conf k) = Some y) \<and> port_of_part conf p (the (cur V (c2s conf k))) 
-            \<longrightarrow> (\<forall>c. c \<noteq> ch_destqport conf p \<longrightarrow> \<acute>qbuf c = qbuf V c \<and> \<acute>qbufsize c = qbufsize V c)) \<and>
-            ((is_dest_qport conf p \<longrightarrow> cur V (c2s conf k) = None \<or> \<not> port_of_part conf p (the (cur V (c2s conf k)))) 
-            \<longrightarrow> \<acute>qbuf = qbuf V \<and> \<acute>qbufsize = qbufsize V)\<rbrace>]"
-  apply(case_tac "is_dest_qport conf p \<and> (\<exists>y. (cur V) ((c2s conf) k) = Some y) 
-                  \<and> port_of_part conf p (the ((cur V) ((c2s conf) k)))\<and> 0 < (qbufsize V) (ch_destqport conf p)")
-   apply simp
-   apply(rule Seq[where mid="{s. s = V\<lparr>qbuf := (qbuf V)(ch_destqport conf p := tl ((qbuf V) (ch_destqport conf p)))\<rparr>}"])
-    apply(rule Basic)
-        apply auto[1]
-       apply auto[1]
-      apply blast
-     apply(simp add: stable_def)+
-   apply(rule Basic, simp)
-      apply auto[1]
-     apply(simp add: stable_def)+
-  apply(rule Seq[where mid="{}"])
-   apply(rule Basic)
-       apply(simp add:stable_def)+
-  apply(rule Basic, simp)
-     apply(simp add:stable_def)+
-  done
-
-lemma Recv_Que_Message_SatRG: " \<Gamma> \<turnstile> Recv_Que_Message k p sat Recv_Que_Message_RGCond k p"
-  apply(simp add:Evt_sat_RG_def)
-  apply(simp add:Recv_Que_Message_def)
-  apply(rule BasicEvt)
-    apply(simp add:body_def Recv_Que_Message_RGCond_def guard_def Pre\<^sub>f_def Post\<^sub>f_def Rely\<^sub>f_def
-          Guar\<^sub>f_def getrgformula_def)
-    apply(rule Await)
-       apply(simp add: stable_def)+
-    apply(rule allI)
-  using Recv_Que_Message_SatRG_h1 apply fastforce
-  apply(simp add: stable_def Recv_Que_Message_RGCond_def Pre\<^sub>f_def Rely\<^sub>f_def getrgformula_def stable_e_def)
-  apply(simp add: Recv_Que_Message_RGCond_def Guar\<^sub>f_def getrgformula_def)
-  done
-
-lemma EvtSys1_on_core_SatRG: 
-  "\<forall>k. \<Gamma> \<turnstile> fst (EvtSys1_on_Core_RGF k) sat\<^sub>s 
-       [Pre\<^sub>f (snd (EvtSys1_on_Core_RGF k)), 
-       Rely\<^sub>f (snd (EvtSys1_on_Core_RGF k)), 
-       Guar\<^sub>f (snd (EvtSys1_on_Core_RGF k)), 
-        Post\<^sub>f (snd (EvtSys1_on_Core_RGF k))]"
-  apply (rule allI)
-  apply(simp add:EvtSys1_on_Core_RGF_def Pre\<^sub>f_def Rely\<^sub>f_def Guar\<^sub>f_def Post\<^sub>f_def getrgformula_def)
-  apply (rule EvtSys_h)
-                    
-  apply(clarify)
-  apply(case_tac "(a,b)\<in> {(Schedule_RGF k x)}")
-  using Sched_SatRG Schedule_RGF_def Evt_sat_RG_def E\<^sub>e_def Pre\<^sub>e_def Rely\<^sub>e_def Guar\<^sub>e_def Post\<^sub>e_def 
-    Guar\<^sub>f_def Post\<^sub>f_def Pre\<^sub>f_def Rely\<^sub>f_def snd_conv fst_conv apply (metis singletonD)
-  apply(case_tac "(a,b)\<in>(\<Union>(p, m). {Send_Que_Message_RGF k p m})")
-  apply(clarify)
-  using Send_Que_Message_SatRG Send_Que_Message_RGF_def E\<^sub>e_def Pre\<^sub>e_def Rely\<^sub>e_def Guar\<^sub>e_def Post\<^sub>e_def 
-    Guar\<^sub>f_def Post\<^sub>f_def Pre\<^sub>f_def Rely\<^sub>f_def snd_conv fst_conv Evt_sat_RG_def apply metis
-  apply(case_tac "(a,b)\<in>(\<Union>p. {Recv_Que_Message_RGF k p})")
-  apply(clarify)
-  using Recv_Que_Message_SatRG Recv_Que_Message_RGF_def E\<^sub>e_def Pre\<^sub>e_def Rely\<^sub>e_def Guar\<^sub>e_def Post\<^sub>e_def 
-    Guar\<^sub>f_def Post\<^sub>f_def Pre\<^sub>f_def Rely\<^sub>f_def snd_conv fst_conv Evt_sat_RG_def apply metis
-  apply blast
-
-  apply(clarify)
-  apply(case_tac "(a,b)\<in> {(Schedule_RGF k x)}")
-  apply(simp add:Schedule_RGF_def Schedule_RGCond_def Pre\<^sub>e_def getrgformula_def)
-  apply(case_tac "(a,b)\<in>(\<Union>(p, m). {Send_Que_Message_RGF k p m})")
-  apply clarify
-  apply(simp add:Send_Que_Message_RGF_def Send_Que_Message_RGCond_def Pre\<^sub>e_def getrgformula_def)
-  apply(case_tac "(a,b)\<in>(\<Union>p. {Recv_Que_Message_RGF k p})")
-  apply(clarify)
-  apply(simp add:Recv_Que_Message_RGF_def Recv_Que_Message_RGCond_def Pre\<^sub>e_def getrgformula_def)
-  apply blast
-
-  apply(clarify)
-  apply(case_tac "(a,b)\<in> {(Schedule_RGF k x)}")
-  apply(simp add:Schedule_RGF_def Schedule_RGCond_def Rely\<^sub>e_def getrgformula_def) 
-  apply(case_tac "(a,b)\<in>(\<Union>(p, m). {Send_Que_Message_RGF k p m})")
-  apply clarify
-  apply(simp add:Send_Que_Message_RGF_def Send_Que_Message_RGCond_def Rely\<^sub>e_def getrgformula_def)
-  apply(case_tac "(a,b)\<in>(\<Union>p. {Recv_Que_Message_RGF k p})")
-  apply(clarify)
-  apply(simp add:Recv_Que_Message_RGF_def Recv_Que_Message_RGCond_def Rely\<^sub>e_def getrgformula_def)
-  apply blast
-
-  apply(clarify)
-  apply(case_tac "(a,b)\<in> {(Schedule_RGF k x)}")
-  apply(simp add:Schedule_RGF_def Schedule_RGCond_def getrgformula_def Guar\<^sub>e_def) 
-  apply auto[1] 
-  apply(case_tac "(a,b)\<in>(\<Union>(p, m). {Send_Que_Message_RGF k p m})")
-  apply(simp add:Send_Que_Message_RGF_def Send_Que_Message_RGCond_def getrgformula_def Guar\<^sub>e_def, clarify)
-  apply auto[1]
-  apply(case_tac "(a,b)\<in>(\<Union>p. {Recv_Que_Message_RGF k p})")
-  apply(simp add:Recv_Que_Message_RGF_def Recv_Que_Message_RGCond_def getrgformula_def Guar\<^sub>e_def) 
-  apply auto[1] 
-  apply blast
-  
-  apply simp
-
-  apply(clarify)
-  apply(case_tac "(a,b)\<in> {(Schedule_RGF k xa)}")
-  apply(case_tac "(aa,ba)\<in> {(Schedule_RGF k xb)}")
-  apply(simp add:Schedule_RGF_def Schedule_RGCond_def getrgformula_def Pre\<^sub>e_def)
-  apply(case_tac "(aa,ba)\<in>(\<Union>(p, m). {Send_Que_Message_RGF k p m})")
-  apply(simp add:Send_Que_Message_RGF_def Send_Que_Message_RGCond_def getrgformula_def Pre\<^sub>e_def)  
-  apply auto[1] 
-  apply(case_tac "(aa,ba)\<in>(\<Union>p. {Recv_Que_Message_RGF k p})")
-  apply(simp add:Recv_Que_Message_RGF_def Recv_Que_Message_RGCond_def getrgformula_def Pre\<^sub>e_def) 
-  apply auto[1] 
-  apply blast
-
-  apply(case_tac "(a,b)\<in>(\<Union>(p, m). {Send_Que_Message_RGF k p m})")
-  apply(case_tac "(aa,ba)\<in> {(Schedule_RGF k xb)}")
-  apply(simp add:Schedule_RGF_def Schedule_RGCond_def getrgformula_def Pre\<^sub>e_def)
-  apply(case_tac "(aa,ba)\<in>(\<Union>(p, m). {Send_Que_Message_RGF k p m})")
-  apply(simp add:Send_Que_Message_RGF_def Send_Que_Message_RGCond_def getrgformula_def Pre\<^sub>e_def) 
-  apply auto[1] 
-  apply(case_tac "(aa,ba)\<in>(\<Union>p. {Recv_Que_Message_RGF k p})")
-  apply(simp add:Recv_Que_Message_RGF_def Recv_Que_Message_RGCond_def getrgformula_def Pre\<^sub>e_def) 
-  apply auto[1] 
-  apply blast
-  apply(case_tac "(a,b)\<in>(\<Union>p. {Recv_Que_Message_RGF k p})")
-  apply(case_tac "(aa,ba)\<in> {(Schedule_RGF k xb)}")
-  apply(simp add:Schedule_RGF_def Schedule_RGCond_def getrgformula_def Pre\<^sub>e_def)
-  apply(case_tac "(aa,ba)\<in>(\<Union>(p, m). {Send_Que_Message_RGF k p m})")
-  apply(simp add:Send_Que_Message_RGF_def Send_Que_Message_RGCond_def getrgformula_def Pre\<^sub>e_def) 
-  apply auto[1] 
-  apply(case_tac "(aa,ba)\<in>(\<Union>p. {Recv_Que_Message_RGF k p})")
-  apply(simp add:Recv_Que_Message_RGF_def Recv_Que_Message_RGCond_def getrgformula_def Pre\<^sub>e_def) 
-  apply auto[1] 
-  apply blast
-  apply blast
-  apply (simp add:stable_e_def)
-  by simp
-
-
-lemma EvtSys_on_core_SatRG: 
-  "\<forall>k.  \<Gamma> \<turnstile> fst (EvtSys_on_Core_RGF k) sat\<^sub>s 
-          [Pre\<^sub>f (snd (EvtSys_on_Core_RGF k)), 
-           Rely\<^sub>f (snd (EvtSys_on_Core_RGF k)), 
-           Guar\<^sub>f (snd (EvtSys_on_Core_RGF k)), 
-           Post\<^sub>f (snd (EvtSys_on_Core_RGF k))]"
-  apply(rule allI)
-  apply(simp add:EvtSys_on_Core_RGF_def Pre\<^sub>f_def Rely\<^sub>f_def Guar\<^sub>f_def Post\<^sub>f_def getrgformula_def)
-  apply(rule EvtSeq_h)
-          apply(simp add:E\<^sub>e_def Core_Init_RGF_def Pre\<^sub>e_def Rely\<^sub>e_def Guar\<^sub>e_def Post\<^sub>e_def)
-          apply (metis Core_Init_SatRG Evt_sat_RG_def Guar\<^sub>f_def Post\<^sub>f_def Pre\<^sub>f_def Rely\<^sub>f_def) 
-  using EvtSys1_on_core_SatRG apply fastforce
-        apply(simp add:Core_Init_RGF_def Core_Init_RGCond_def Pre\<^sub>e_def getrgformula_def) 
-       apply(simp add:EvtSys1_on_Core_RGF_def Post\<^sub>f_def getrgformula_def)
-      apply(simp add:Core_Init_RGF_def Core_Init_RGCond_def Rely\<^sub>e_def getrgformula_def) 
-      apply auto[1]
-     apply(simp add:EvtSys1_on_Core_RGF_def Rely\<^sub>f_def getrgformula_def Core_Init_RGF_def)
-    apply(simp add:Core_Init_RGF_def Core_Init_RGCond_def Guar\<^sub>e_def Guar\<^sub>f_def getrgformula_def EvtSys1_on_Core_RGF_def)
-   apply(simp add:EvtSys1_on_Core_RGF_def Core_Init_RGCond_def Guar\<^sub>f_def getrgformula_def)
-  by (simp add:EvtSys1_on_Core_RGF_def Core_Init_RGF_def Core_Init_RGCond_def Post\<^sub>e_def Pre\<^sub>f_def getrgformula_def)
-
-lemma spec_sat_rg: "\<forall>k. \<Gamma> \<turnstile> fst (ARINCXKernel_Spec k) sat\<^sub>s [Pre\<^sub>e\<^sub>s (ARINCXKernel_Spec k),
-           Rely\<^sub>e\<^sub>s (ARINCXKernel_Spec k), Guar\<^sub>e\<^sub>s (ARINCXKernel_Spec k), Post\<^sub>e\<^sub>s (ARINCXKernel_Spec k)]"
-  apply (simp add:ARINCXKernel_Spec_def Guar\<^sub>e\<^sub>s_def Guar\<^sub>f_def Post\<^sub>e\<^sub>s_def Post\<^sub>f_def Pre\<^sub>e\<^sub>s_def  Pre\<^sub>f_def Rely\<^sub>e\<^sub>s_def Rely\<^sub>f_def)
-  by (metis EvtSys_on_core_SatRG Guar\<^sub>f_def Post\<^sub>f_def Pre\<^sub>f_def Rely\<^sub>f_def)
-
-lemma spec_sat_init: "\<forall>k. {s0} \<subseteq> Pre\<^sub>e\<^sub>s (ARINCXKernel_Spec k)"
-  by(simp add:ARINCXKernel_Spec_def EvtSys_on_Core_RGF_def Pre\<^sub>e\<^sub>s_def getrgformula_def System_Init_def s0_init)
-
-lemma spec_rg_com: "\<forall>k j. j \<noteq> k \<longrightarrow> Guar\<^sub>e\<^sub>s (ARINCXKernel_Spec j) \<subseteq> Rely\<^sub>e\<^sub>s (ARINCXKernel_Spec k)"
-  apply (clarsimp)
-  apply(simp add:ARINCXKernel_Spec_def EvtSys_on_Core_RGF_def Guar\<^sub>e\<^sub>s_def Rely\<^sub>e\<^sub>s_def getrgformula_def)  
-  apply auto[1]
-    apply (simp add: inj_eq inj_surj_c2s)
-   apply (metis inj_eq inj_surj_c2s)
-  by metis
-
-
-
-subsection \<open>Security Specification\<close>
-
-datatype Domain = P Part | S Sched | F 
-
-
-definition domevt :: "State  \<Rightarrow> (EventLabel, Core, State, Prog) event \<Rightarrow> Domain"
-  where "domevt s e \<equiv> let c = get_evt_core e in (let el = get_evt_el e in  
-                         (if (el = Send_Que_MessageE \<or> el = Recv_Que_MessageE) 
-                              \<and> (cur s) (c2s conf c) \<noteq> None
-                              then P (the ((cur s) (c2s conf c)))
-                          else if (el = Core_InitE \<or> el = ScheduleE) then S (c2s conf c)
-                          else F))" 
 
 primrec part_on_core :: "Config \<Rightarrow> Domain \<Rightarrow> Domain \<Rightarrow> bool"
   where "part_on_core cfg (P d1) d2 = (case d2 of
@@ -634,752 +90,1042 @@ definition interf :: "Domain \<Rightarrow> Domain \<Rightarrow> bool" ("(_ \<lea
 definition noninterf :: "Domain \<Rightarrow> Domain \<Rightarrow> bool" ("(_ \<setminus>\<leadsto> _)" [70,71] 60)
   where "u \<setminus>\<leadsto> v \<equiv> \<not> (u \<leadsto> v)"
 
-definition state_obs_sched :: "State \<Rightarrow> Sched \<Rightarrow> State"
-  where "state_obs_sched s d \<equiv> s0\<lparr>cur:=(cur s0) (d := (cur s) d)\<rparr>"
+subsubsection \<open>Implementation Specification\<close>
 
-definition obs_cap_part :: "State \<Rightarrow> Part  \<Rightarrow> (QChannel \<Rightarrow> nat)"
-  where "obs_cap_part s p  \<equiv> \<lambda>c. if (p2p conf) ((chdest conf) c) = p then qbufsize s c else qbufsize s0 c"
+record State\<^sub>c = cur\<^sub>c :: "Sched \<Rightarrow> Part option"
+                qlock\<^sub>c :: "QChannel \<Rightarrow> Core option"
+                qbuf\<^sub>c :: "QChannel \<Rightarrow> Message list"
+                qbufsize\<^sub>c :: "QChannel \<Rightarrow> nat"
+                obsize\<^sub>c :: "QChannel \<Rightarrow> nat"
+                partst\<^sub>c :: "Part \<Rightarrow> PartMode"
 
-lemma obs_cap_equiv : "\<lbrakk>\<forall>c. p2p conf (chdest conf c) = x1 \<longrightarrow> qbufsize s1 c = qbufsize s2 c\<rbrakk> 
-                        \<Longrightarrow>  obs_cap_part s2 x1 = obs_cap_part s1 x1"
-  apply (simp add: obs_cap_part_def)
+type_synonym Prog\<^sub>c = "State\<^sub>c com option"
+
+definition Core_Init\<^sub>c :: "Core \<Rightarrow> (EventLabel, Core, State\<^sub>c, Prog\<^sub>c) event" 
+  where "Core_Init\<^sub>c k \<equiv> 
+    EVENT Core_InitE [] \<rhd> k 
+    THEN      
+      \<acute>partst\<^sub>c := (\<lambda>p. if p2s conf p = c2s conf k \<and> \<acute>partst\<^sub>c p = IDLE then READY else \<acute>partst\<^sub>c p) 
+    END"
+
+definition System_Init\<^sub>c :: "Config \<Rightarrow> (State\<^sub>c \<times> (EventLabel, Core, State\<^sub>c, Prog\<^sub>c) x)"
+  where "System_Init\<^sub>c cfg \<equiv> (\<lparr>cur\<^sub>c=(\<lambda>s. None),
+                            qlock\<^sub>c = (\<lambda>c. None),
+                            qbuf\<^sub>c = (\<lambda>c. []),
+                            qbufsize\<^sub>c = (\<lambda>c. 0),
+                            obsize\<^sub>c = (\<lambda>c. 0),
+                            partst\<^sub>c = (\<lambda>p. IDLE)\<rparr>, 
+                            (\<lambda>k. Core_Init\<^sub>c k))"
+
+definition Schedule\<^sub>c :: "Core \<Rightarrow> Part \<Rightarrow> (EventLabel, Core, State\<^sub>c, Prog\<^sub>c) event" 
+  where "Schedule\<^sub>c k p \<equiv> 
+    EVENT ScheduleE [Partition p] \<rhd> k 
+    WHERE
+      p2s conf p = c2s conf k \<and> (\<acute>partst\<^sub>c p \<noteq> IDLE) \<and> (\<acute>cur\<^sub>c (c2s conf k) = None 
+          \<or> p2s conf (the (\<acute>cur\<^sub>c((c2s conf) k))) = c2s conf k)
+    THEN
+        ATOMIC
+          IF (\<acute>cur\<^sub>c((c2s conf) k) \<noteq> None) THEN    
+           \<acute>partst\<^sub>c := \<acute>partst\<^sub>c(the (\<acute>cur\<^sub>c ((c2s conf) k)) := READY);;
+           \<acute>cur\<^sub>c := \<acute>cur\<^sub>c((c2s conf) k := None)
+          FI;;
+         \<acute>cur\<^sub>c := \<acute>cur\<^sub>c((c2s conf k) := Some p);;
+         \<acute>partst\<^sub>c := \<acute>partst\<^sub>c(p := RUN)
+        END
+    END"
+
+definition Send_Que_Message\<^sub>c :: "Core \<Rightarrow> Port \<Rightarrow> Message \<Rightarrow> (EventLabel, Core, State\<^sub>c, Prog\<^sub>c) event" 
+  where "Send_Que_Message\<^sub>c k p m \<equiv> 
+    EVENT Send_Que_MessageE [Port p, Message m] \<rhd> k 
+    WHERE
+      is_src_qport conf p
+      \<and> \<acute>cur\<^sub>c (c2s conf k) \<noteq> None
+      \<and> port_of_part conf p (the (\<acute>cur\<^sub>c (c2s conf k)))
+    THEN
+      AWAIT \<acute>qlock\<^sub>c (ch_srcqport conf p) = None THEN
+        \<acute>qlock\<^sub>c := \<acute>qlock\<^sub>c (ch_srcqport conf p := Some k)
+      END;;
+      IF \<acute>qbufsize\<^sub>c (ch_srcqport conf p) < chmax conf (ch_srcqport conf p) THEN 
+        \<acute>qbuf\<^sub>c := \<acute>qbuf\<^sub>c (ch_srcqport conf p := \<acute>qbuf\<^sub>c (ch_srcqport conf p) @ [m]);;
+        \<acute>qbufsize\<^sub>c := \<acute>qbufsize\<^sub>c (ch_srcqport conf p := \<acute>qbufsize\<^sub>c (ch_srcqport conf p) + 1)
+      FI;;
+      ATOMIC
+        \<acute>qlock\<^sub>c := \<acute>qlock\<^sub>c (ch_srcqport conf p := None);;
+        \<acute>obsize\<^sub>c := \<acute>obsize\<^sub>c (ch_srcqport conf p := \<acute>qbufsize\<^sub>c (ch_srcqport conf p))
+      END   
+    END"
+
+definition Recv_Que_Message\<^sub>c :: "Core \<Rightarrow> Port \<Rightarrow> (EventLabel, Core, State\<^sub>c, Prog\<^sub>c) event" 
+  where "Recv_Que_Message\<^sub>c k p \<equiv> 
+    EVENT Recv_Que_MessageE [Port p] \<rhd> k 
+    WHERE
+      is_dest_qport conf p 
+      \<and> \<acute>cur\<^sub>c (c2s conf k) \<noteq> None
+      \<and> port_of_part conf p (the (\<acute>cur\<^sub>c (c2s conf k)))
+    THEN 
+      AWAIT \<acute>qlock\<^sub>c (ch_destqport conf p) = None THEN
+        \<acute>qlock\<^sub>c := \<acute>qlock\<^sub>c (ch_destqport conf p := Some k)
+      END;;
+      IF \<acute>qbufsize\<^sub>c (ch_destqport conf p) > 0 THEN 
+        \<acute>qbuf\<^sub>c := \<acute>qbuf\<^sub>c (ch_destqport conf p := tl (\<acute>qbuf\<^sub>c (ch_destqport conf p)));;
+        \<acute>qbufsize\<^sub>c := \<acute>qbufsize\<^sub>c (ch_destqport conf p := \<acute>qbufsize\<^sub>c (ch_destqport conf p) - 1)
+      FI;;
+      ATOMIC
+        \<acute>qlock\<^sub>c := \<acute>qlock\<^sub>c (ch_destqport conf p := None);;
+        \<acute>obsize\<^sub>c := \<acute>obsize\<^sub>c (ch_destqport conf p := \<acute>qbufsize\<^sub>c (ch_destqport conf p))
+      END
+    END"
+
+
+definition EvtSys_on_Core\<^sub>c :: "Core \<Rightarrow> (EventLabel, Core, State\<^sub>c, Prog\<^sub>c) esys"
+  where "EvtSys_on_Core\<^sub>c k = EvtSeq (Core_Init\<^sub>c k) (EvtSys
+  (\<Union>p.{Schedule\<^sub>c k p} \<union> (\<Union>(p, m). {Send_Que_Message\<^sub>c k p m}) \<union> (\<Union>p.{Recv_Que_Message\<^sub>c k p})))"
+
+definition ARINCXKernel_Spec\<^sub>c :: "(EventLabel, Core, State\<^sub>c, Prog\<^sub>c) paresys"
+  where "ARINCXKernel_Spec\<^sub>c \<equiv> (\<lambda>k. EvtSys_on_Core\<^sub>c k)"
+
+axiomatization s0\<^sub>c where s0c_init: "s0\<^sub>c \<equiv> fst (System_Init\<^sub>c conf)"
+axiomatization x0\<^sub>c where x0c_init: "x0\<^sub>c \<equiv> snd (System_Init\<^sub>c conf)"
+axiomatization C0\<^sub>c where C0c_init: "C0\<^sub>c = (ARINCXKernel_Spec\<^sub>c, s0\<^sub>c, x0\<^sub>c)"
+
+definition domevt\<^sub>c :: "State\<^sub>c \<Rightarrow> (EventLabel, Core, State\<^sub>c, Prog\<^sub>c) event \<Rightarrow> Domain"
+  where "domevt\<^sub>c s e \<equiv> let c = get_evt_core e in (let el = get_evt_el e in  
+                         (if (el = Send_Que_MessageE \<or> el = Recv_Que_MessageE) 
+                              \<and> (cur\<^sub>c s) (c2s conf c) \<noteq> None
+                              then P (the ((cur\<^sub>c s) (c2s conf c)))
+                          else if (el = Core_InitE \<or> el = ScheduleE) then S (c2s conf c)
+                          else F))" 
+
+definition exec_step\<^sub>c :: "'Env \<Rightarrow> (EventLabel, Core, State\<^sub>c, Prog\<^sub>c, Domain) action \<Rightarrow> 
+ ((EventLabel, Core, State\<^sub>c, Prog\<^sub>c) pesconf \<times> (EventLabel, Core, State\<^sub>c, Prog\<^sub>c) pesconf) set"
+  where "exec_step\<^sub>c \<Gamma>\<^sub>c a \<equiv> {(P,Q). (\<Gamma>\<^sub>c \<turnstile>\<^sub>c P-pes-(actk a)\<rightarrow> Q) \<and>((\<exists>e k. actk a = ((EvtEnt e)\<sharp>k) \<and> eventof a = e 
+                         \<and> domevt\<^sub>c (gets P) e = domain a) \<or> (\<exists>c k. actk a = ((Cmd c)\<sharp>k) 
+                         \<and> eventof a = (getx P) k \<and> domevt\<^sub>c (gets P) (eventof a) = domain a))}"
+
+definition state_obs_sched\<^sub>c :: "State\<^sub>c \<Rightarrow> Sched \<Rightarrow> State\<^sub>c"
+  where "state_obs_sched\<^sub>c s d \<equiv> s0\<^sub>c\<lparr>cur\<^sub>c :=(cur\<^sub>c s0\<^sub>c) (d := (cur\<^sub>c s) d)\<rparr>"
+
+definition obs_cap_part\<^sub>c :: "State\<^sub>c \<Rightarrow> Part \<Rightarrow> (QChannel \<Rightarrow> nat)"
+  where "obs_cap_part\<^sub>c s p  \<equiv> \<lambda>c. if (p2p conf) ((chdest conf) c) = p then obsize\<^sub>c s c else obsize\<^sub>c s0\<^sub>c c"
+
+lemma obs_cap_equivc : "\<lbrakk>\<forall>c. p2p conf (chdest conf c) = x1 \<longrightarrow> obsize\<^sub>c s1 c = obsize\<^sub>c s2 c\<rbrakk> 
+                        \<Longrightarrow>  obs_cap_part\<^sub>c s2 x1 = obs_cap_part\<^sub>c s1 x1"
+  apply (simp add: obs_cap_part\<^sub>c_def)
   by force
 
-lemma obs_cap_equiv1 : "qbufsize s1 = qbufsize s2 \<Longrightarrow> obs_cap_part s1 p = obs_cap_part s2 p"
-  using obs_cap_equiv by force
+definition state_obs_part\<^sub>c :: "State\<^sub>c \<Rightarrow> Part \<Rightarrow> State\<^sub>c"
+  where "state_obs_part\<^sub>c s p \<equiv> s0\<^sub>c\<lparr>partst\<^sub>c := (partst\<^sub>c s0\<^sub>c) (p := (partst\<^sub>c s) p), 
+                                  obsize\<^sub>c := obs_cap_part\<^sub>c s p\<rparr>"
 
-definition state_obs_part :: "State \<Rightarrow> Part \<Rightarrow> State"
-  where "state_obs_part s p \<equiv> s0\<lparr>partst := (partst s0) (p := (partst s) p), 
-                                 qbufsize := obs_cap_part s p\<rparr>"
+primrec state_obs\<^sub>c :: "State\<^sub>c \<Rightarrow> Domain \<Rightarrow> State\<^sub>c"
+  where "state_obs\<^sub>c s (P p) = state_obs_part\<^sub>c s p" |
+        "state_obs\<^sub>c s (S p) = state_obs_sched\<^sub>c s p"|
+        "state_obs\<^sub>c s F = s0\<^sub>c"
 
-primrec state_obs :: "State \<Rightarrow> Domain \<Rightarrow> State"
-  where "state_obs s (P p) = state_obs_part s p" |
-        "state_obs s (S p) = state_obs_sched s p"|
-        "state_obs s F = s0"
+definition state_equiv\<^sub>c :: "State\<^sub>c \<Rightarrow> Domain \<Rightarrow> State\<^sub>c \<Rightarrow> bool" ("(_ \<sim>\<^sub>c_\<sim>\<^sub>c _)" [70,69,70] 60)
+  where "state_equiv\<^sub>c s d t \<equiv> state_obs\<^sub>c s d = state_obs\<^sub>c t d"
 
-definition state_equiv :: "State \<Rightarrow> Domain \<Rightarrow> State \<Rightarrow> bool" ("(_ \<sim>_\<sim> _)" [70,69,70] 60)
-  where "state_equiv s d t \<equiv> state_obs s d = state_obs t d"
-
-lemma state_equiv_transitive: "\<lbrakk>s \<sim> d \<sim> t; t \<sim> d \<sim> r\<rbrakk> \<Longrightarrow> s \<sim> d \<sim> r"
-  by (simp add:state_equiv_def)
+lemma state_equiv_transitivec: "\<lbrakk>s \<sim>\<^sub>c d \<sim>\<^sub>c t; t \<sim>\<^sub>c d \<sim>\<^sub>c r\<rbrakk> \<Longrightarrow> s \<sim>\<^sub>c d \<sim>\<^sub>c r"
+  by (simp add:state_equiv\<^sub>c_def)
     
-lemma state_equiv_symmetric : "s \<sim> d \<sim> t \<Longrightarrow> t \<sim> d \<sim> s"
-  by (simp add:state_equiv_def)
+lemma state_equiv_symmetricc : "s \<sim>\<^sub>c d \<sim>\<^sub>c t \<Longrightarrow> t \<sim>\<^sub>c d \<sim>\<^sub>c s"
+  by (simp add:state_equiv\<^sub>c_def)
 
-lemma state_equiv_reflexive : "s \<sim> d \<sim> s"
-  by (simp add:state_equiv_def)
-
-
-definition exec_step :: "'Env \<Rightarrow> (EventLabel, Core, State, Prog, Domain) action \<Rightarrow> 
- ((EventLabel, Core, State, Prog) pesconf \<times> (EventLabel, Core, State, Prog) pesconf) set"
-  where "exec_step \<Gamma> a \<equiv> {(P,Q). (\<Gamma> \<turnstile> P-pes-(actk a)\<rightarrow> Q) \<and>((\<exists>e k. actk a = ((EvtEnt e)\<sharp>k) \<and> eventof a = e 
-                         \<and> domevt (gets P) e = domain a) \<or> (\<exists>c k. actk a = ((Cmd c)\<sharp>k) 
-                         \<and> eventof a = (getx P) k \<and> domevt (gets P) (eventof a) = domain a))}"
+lemma state_equiv_reflexivec : "s \<sim>\<^sub>c d \<sim>\<^sub>c s"
+  by (simp add:state_equiv\<^sub>c_def)
 
 
-subsection \<open>Instantiate the Security Model\<close>
+subsubsection \<open>Abstraction Specification\<close>
 
-lemma neq_coreinit: "k1\<noteq>k2 \<Longrightarrow> Core_Init k1\<noteq>Core_Init k2" 
-  by (simp add:Core_Init_def get_evt_label_def)
+record State\<^sub>a = cur\<^sub>a :: "Sched \<Rightarrow> Part option"
+                qbuf\<^sub>a :: "QChannel \<Rightarrow> Message list"
+                qbufsize\<^sub>a :: "QChannel \<Rightarrow> nat"              
+                partst\<^sub>a :: "Part \<Rightarrow> PartMode"
 
-lemma neq_schedule: " k1 \<noteq> k2 \<or> p1 \<noteq> p2 \<Longrightarrow> Schedule k1 p1 \<noteq>Schedule k2 p2" 
-  by (simp add:Schedule_def get_evt_label_def)
+type_synonym Prog\<^sub>a = "State\<^sub>a com option"
 
-lemma neq_wrt_samp: " k1\<noteq>k2 \<or> p1\<noteq>p2 \<or> m1\<noteq>m2 \<Longrightarrow> Send_Que_Message k1 p1 m1 \<noteq> Send_Que_Message k2 p2 m2" 
-  by (clarsimp, simp add: Send_Que_Message_def get_evt_label_def)
+definition Core_Init\<^sub>a :: "Core \<Rightarrow> (EventLabel, Core, State\<^sub>a, Prog\<^sub>a) event" 
+  where "Core_Init\<^sub>a k \<equiv> 
+    EVENT Core_InitE [] \<rhd> k 
+    THEN      
+      \<acute>partst\<^sub>a := (\<lambda>p. if p2s conf p = c2s conf k \<and> \<acute>partst\<^sub>a p = IDLE then READY else \<acute>partst\<^sub>a p)
+    END"
 
-lemma neq_rd_samp: "k1\<noteq>k2 \<or> p1\<noteq>p2 \<Longrightarrow> Recv_Que_Message k1 p1 \<noteq> Recv_Que_Message k2 p2" 
-  by (clarsimp, simp add: Recv_Que_Message_def get_evt_label_def)
+definition System_Init\<^sub>a :: "Config \<Rightarrow> (State\<^sub>a \<times> (EventLabel, Core, State\<^sub>a, Prog\<^sub>a) x)"
+  where "System_Init\<^sub>a cfg \<equiv> (\<lparr>cur\<^sub>a=(\<lambda>s. None),
+                            qbuf\<^sub>a = (\<lambda>c. []),
+                            qbufsize\<^sub>a = (\<lambda>c. 0),
+                            partst\<^sub>a = (\<lambda>p. IDLE)\<rparr>, 
+                            (\<lambda>k. Core_Init\<^sub>a k))"
 
-lemma neq_coreinit_sched: "Core_Init k1 \<noteq> Schedule k2 p"
-  by (simp add:Schedule_def Core_Init_def get_evt_label_def)
+definition Schedule\<^sub>a :: "Core \<Rightarrow> Part \<Rightarrow> (EventLabel, Core, State\<^sub>a, Prog\<^sub>a) event" 
+  where "Schedule\<^sub>a k p \<equiv> 
+    EVENT ScheduleE [Partition p] \<rhd> k 
+    WHERE
+      p2s conf p = c2s conf k \<and> (\<acute>partst\<^sub>a p \<noteq> IDLE) \<and> (\<acute>cur\<^sub>a (c2s conf k) = None 
+          \<or> p2s conf (the (\<acute>cur\<^sub>a((c2s conf) k))) = c2s conf k)
+    THEN
+        ATOMIC
+          IF (\<acute>cur\<^sub>a((c2s conf) k) \<noteq> None) THEN    
+           \<acute>partst\<^sub>a := \<acute>partst\<^sub>a(the (\<acute>cur\<^sub>a ((c2s conf) k)) := READY)
+          FI;;
+         \<acute>cur\<^sub>a := \<acute>cur\<^sub>a((c2s conf k) := Some p);;
+         \<acute>partst\<^sub>a := \<acute>partst\<^sub>a(p := RUN)
+        END
+    END"
 
-lemma neq_coreinit_wrtsamp: "Core_Init k1 \<noteq> Send_Que_Message k2 p m"
-  by (simp add:Send_Que_Message_def Core_Init_def get_evt_label_def)
+definition Send_Que_Message\<^sub>a :: "Core \<Rightarrow> Port \<Rightarrow> Message \<Rightarrow> (EventLabel, Core, State\<^sub>a, Prog\<^sub>a) event" 
+  where "Send_Que_Message\<^sub>a k p m \<equiv> 
+    EVENT Send_Que_MessageE [Port p, Message m] \<rhd> k 
+    WHERE
+      is_src_qport conf p
+      \<and> \<acute>cur\<^sub>a (c2s conf k) \<noteq> None
+      \<and> port_of_part conf p (the (\<acute>cur\<^sub>a (c2s conf k)))
+    THEN
+      ATOMIC
+        IF \<acute>qbufsize\<^sub>a (ch_srcqport conf p) < chmax conf (ch_srcqport conf p) THEN 
+          \<acute>qbuf\<^sub>a := \<acute>qbuf\<^sub>a (ch_srcqport conf p := \<acute>qbuf\<^sub>a (ch_srcqport conf p) @ [m]);;
+          \<acute>qbufsize\<^sub>a := \<acute>qbufsize\<^sub>a (ch_srcqport conf p := \<acute>qbufsize\<^sub>a (ch_srcqport conf p) + 1)
+        FI
+      END  
+    END"
 
-lemma neq_coreinit_rdsamp: "Core_Init k1 \<noteq> Recv_Que_Message k2 p"
-  by (simp add:Recv_Que_Message_def Core_Init_def get_evt_label_def)
+definition Recv_Que_Message\<^sub>a :: "Core \<Rightarrow> Port \<Rightarrow> (EventLabel, Core, State\<^sub>a, Prog\<^sub>a) event" 
+  where "Recv_Que_Message\<^sub>a k p \<equiv> 
+    EVENT Recv_Que_MessageE [Port p] \<rhd> k 
+    WHERE
+      is_dest_qport conf p 
+      \<and> \<acute>cur\<^sub>a (c2s conf k) \<noteq> None
+      \<and> port_of_part conf p (the (\<acute>cur\<^sub>a (c2s conf k)))
+    THEN 
+      ATOMIC
+        IF \<acute>qbufsize\<^sub>a (ch_destqport conf p) > 0 THEN 
+        \<acute>qbuf\<^sub>a := \<acute>qbuf\<^sub>a (ch_destqport conf p := tl (\<acute>qbuf\<^sub>a (ch_destqport conf p)));;
+        \<acute>qbufsize\<^sub>a := \<acute>qbufsize\<^sub>a (ch_destqport conf p := \<acute>qbufsize\<^sub>a (ch_destqport conf p) - 1)
+        FI
+      END
+    END"
 
-lemma neq_sched_wrtsamp: "Schedule k1 p1 \<noteq> Send_Que_Message k2 p2 m"
-  by (simp add:Send_Que_Message_def Schedule_def get_evt_label_def)
+definition EvtSys_on_Core\<^sub>a :: "Core \<Rightarrow> (EventLabel, Core, State\<^sub>a, Prog\<^sub>a) esys"
+  where "EvtSys_on_Core\<^sub>a k = EvtSeq (Core_Init\<^sub>a k) (EvtSys
+  (\<Union>p.{Schedule\<^sub>a k p} \<union> (\<Union>(p, m). {Send_Que_Message\<^sub>a k p m}) \<union> (\<Union>p.{Recv_Que_Message\<^sub>a k p})))"
 
-lemma neq_sched_rdsamp: "Schedule k1 p1 \<noteq> Recv_Que_Message k2 p2"
-  by (simp add:Recv_Que_Message_def Schedule_def get_evt_label_def)
+definition ARINCXKernel_Spec\<^sub>a :: "(EventLabel, Core, State\<^sub>a, Prog\<^sub>a) paresys"
+  where "ARINCXKernel_Spec\<^sub>a \<equiv> (\<lambda>k. EvtSys_on_Core\<^sub>a k)"
 
-lemma neq_wrtsamp_rdsamp: "Send_Que_Message k1 p1 m \<noteq> Recv_Que_Message k2 p2"
-  by (simp add:Recv_Que_Message_def Send_Que_Message_def get_evt_label_def)
+axiomatization s0\<^sub>a where s0a_init: "s0\<^sub>a \<equiv> fst (System_Init\<^sub>a conf)"
+axiomatization x0\<^sub>a where x0a_init: "x0\<^sub>a \<equiv> snd (System_Init\<^sub>a conf)"
+axiomatization C0\<^sub>a where C0a_init: "C0\<^sub>a = (ARINCXKernel_Spec\<^sub>a, s0\<^sub>a, x0\<^sub>a)"
 
-definition evtrgfset :: "((EventLabel, Core, State, Prog) event \<times> (State rgformula)) set"
-  where "evtrgfset \<equiv> (\<Union>k.{(Core_Init k, Core_Init_RGCond k)})
-                   \<union> (\<Union>(k, p).{(Schedule k p, Schedule_RGCond k p)})
-                   \<union> (\<Union>(k, p, m).{(Send_Que_Message k p m, Send_Que_Message_RGCond k p m)})
-                   \<union> (\<Union>(k, p).{(Recv_Que_Message k p, Recv_Que_Message_RGCond k p)})"
+definition domevt\<^sub>a :: "State\<^sub>a \<Rightarrow> (EventLabel, Core, State\<^sub>a, Prog\<^sub>a) event \<Rightarrow> Domain"
+  where "domevt\<^sub>a s e \<equiv> let c = get_evt_core e in (let el = get_evt_el e in  
+                         (if (el = Send_Que_MessageE \<or> el = Recv_Que_MessageE) 
+                              \<and> (cur\<^sub>a s) (c2s conf c) \<noteq> None
+                              then P (the ((cur\<^sub>a s) (c2s conf c)))
+                          else if (el = Core_InitE \<or> el = ScheduleE) then S (c2s conf c)
+                          else F))" 
 
-lemma evtrgfset_eq_allevts_ARINCSpec: "all_evts ARINCXKernel_Spec = evtrgfset"
-  proof -
-    have "all_evts ARINCXKernel_Spec = (\<Union>k. all_evts_es (fst (ARINCXKernel_Spec k)))" 
-      by (simp add:all_evts_def)
-    then have "all_evts ARINCXKernel_Spec = (\<Union>k. all_evts_es (fst (EvtSys_on_Core_RGF k)))"
-      by (simp add:ARINCXKernel_Spec_def)
-    then have "all_evts ARINCXKernel_Spec = (\<Union>k. all_evts_es (rgf_EvtSeq (Core_Init_RGF k) (EvtSys1_on_Core_RGF k)))"
-      by (simp add:EvtSys_on_Core_RGF_def)
-    then have "all_evts ARINCXKernel_Spec = (\<Union>k. {Core_Init_RGF k} \<union> (all_evts_es (fst (EvtSys1_on_Core_RGF k))))"
-      by simp
-    then have "all_evts ARINCXKernel_Spec = (\<Union>k. {Core_Init_RGF k} \<union>
-                                                  (\<Union>p. {Schedule_RGF k p} \<union>
-                                                  (\<Union>(p, m). {Send_Que_Message_RGF k p m}) \<union>
-                                                  (\<Union>p.{Recv_Que_Message_RGF k p})))"
-      by (simp add:Core_Init_RGF_def EvtSys1_on_Core_RGF_def)
-    then have "all_evts ARINCXKernel_Spec = (\<Union>k. {(Core_Init k, Core_Init_RGCond k)} \<union>
-                                                  (\<Union>p. {(Schedule k p, Schedule_RGCond k p)} \<union>
-                                                  (\<Union>(p, m). {(Send_Que_Message k p m, Send_Que_Message_RGCond k p m)}) \<union>
-                                                  (\<Union>p.{(Recv_Que_Message k p, Recv_Que_Message_RGCond k p)})))"
-      by (simp add: Core_Init_RGF_def Schedule_RGF_def Send_Que_Message_RGF_def Recv_Que_Message_RGF_def)
-    moreover
-    have "(\<Union>k. {(Core_Init k, Core_Init_RGCond k)} \<union>
-          (\<Union>p. {(Schedule k p, Schedule_RGCond k p)} \<union>
-          (\<Union>(p, m). {(Send_Que_Message k p m, Send_Que_Message_RGCond k p m)}) \<union>
-          (\<Union>p.{(Recv_Que_Message k p, Recv_Que_Message_RGCond k p)}))) = 
-          (\<Union>k. {(Core_Init k, Core_Init_RGCond k)}) \<union>
-          (\<Union>k. (\<Union>p.{(Schedule k p, Schedule_RGCond k p)})) \<union>
-          (\<Union>k. (\<Union>(p, m). {(Send_Que_Message k p m, Send_Que_Message_RGCond k p m)})) \<union>
-          (\<Union>k. (\<Union>p.{(Recv_Que_Message k p, Recv_Que_Message_RGCond k p)}))"
-      by auto
-    moreover
-    have "(\<Union>k. (\<Union>p.{(Schedule k p, Schedule_RGCond k p)}))
-          = (\<Union>(k,p).{(Schedule k p, Schedule_RGCond k p)})" by blast
-    moreover
-    have "(\<Union>k. (\<Union>(p, m). {(Send_Que_Message k p m, Send_Que_Message_RGCond k p m)}))
-          = (\<Union>(k, p, m). {(Send_Que_Message k p m, Send_Que_Message_RGCond k p m)})" by blast
-    moreover
-    have "(\<Union>k. (\<Union>p.{(Recv_Que_Message k p, Recv_Que_Message_RGCond k p)}))
-          = (\<Union>(k,p).{(Recv_Que_Message k p, Recv_Que_Message_RGCond k p)})" by blast
-    ultimately show ?thesis using evtrgfset_def by presburger
-  qed
+definition exec_step\<^sub>a :: "'Env \<Rightarrow> (EventLabel, Core, State\<^sub>a, Prog\<^sub>a, Domain) action \<Rightarrow> 
+ ((EventLabel, Core, State\<^sub>a, Prog\<^sub>a) pesconf \<times> (EventLabel, Core, State\<^sub>a, Prog\<^sub>a) pesconf) set"
+  where "exec_step\<^sub>a \<Gamma>\<^sub>a a \<equiv> {(P,Q). (\<Gamma>\<^sub>a \<turnstile>\<^sub>a P-pes-(actk a)\<rightarrow> Q) \<and>((\<exists>e k. actk a = ((EvtEnt e)\<sharp>k) \<and> eventof a = e 
+                         \<and> domevt\<^sub>a (gets P) e = domain a) \<or> (\<exists>c k. actk a = ((Cmd c)\<sharp>k) 
+                         \<and> eventof a = (getx P) k \<and> domevt\<^sub>a (gets P) (eventof a) = domain a))}"
 
-definition evtrgffun :: "(EventLabel, Core, State, Prog) event \<Rightarrow> (State rgformula) option"
-  where "evtrgffun \<equiv> (\<lambda>e. Some (SOME rg. (e, rg)\<in>evtrgfset))"
+definition state_obs_sched\<^sub>a :: "State\<^sub>a \<Rightarrow> Sched \<Rightarrow> State\<^sub>a"
+  where "state_obs_sched\<^sub>a s d \<equiv> s0\<^sub>a\<lparr>cur\<^sub>a :=(cur\<^sub>a s0\<^sub>a) (d := (cur\<^sub>a s) d)\<rparr>"
 
-lemma evtrgffun_exist: "\<forall>e\<in>Domain evtrgfset. \<exists>ef\<in>evtrgfset. E\<^sub>e ef = e \<and> evtrgffun e = Some (snd ef)"
-  by (metis Domain_iff E\<^sub>e_def evtrgffun_def fst_conv snd_conv someI_ex)
+definition obs_cap_part\<^sub>a :: "State\<^sub>a \<Rightarrow> Part \<Rightarrow> (QChannel \<Rightarrow> nat)"
+  where "obs_cap_part\<^sub>a s p  \<equiv> \<lambda>c. if (p2p conf) ((chdest conf) c) = p then qbufsize\<^sub>a s c else qbufsize\<^sub>a s0\<^sub>a c"
 
-lemma diff_e_in_evtrgfset: "\<forall>ef1 ef2. ef1\<in>evtrgfset \<and> ef2\<in>evtrgfset \<and> ef1\<noteq>ef2 \<longrightarrow> E\<^sub>e ef1 \<noteq> E\<^sub>e ef2"
-  apply(rule allI)+
-  apply(case_tac "ef1\<in>(\<Union>k.{(Core_Init k, Core_Init_RGCond k)})")
-   apply(case_tac "ef2 \<in> (\<Union>k. {(Core_Init k, Core_Init_RGCond k)})")
-    apply (metis (no_types, lifting) E\<^sub>e_def UN_E neq_coreinit prod.sel(1) singletonD)
-   apply(case_tac "ef2 \<in> (\<Union>(k, p).{(Schedule k p, Schedule_RGCond k p)})")
-    apply(clarify) using neq_coreinit_sched apply (simp add:E\<^sub>e_def)
-   apply(case_tac "ef2 \<in> (\<Union>(k, p, m).{(Send_Que_Message k p m, Send_Que_Message_RGCond k p m)})")
-    apply(clarify) using neq_coreinit_wrtsamp apply (simp add:E\<^sub>e_def)
-   apply(case_tac "ef2 \<in> (\<Union>(k, p).{(Recv_Que_Message k p, Recv_Que_Message_RGCond k p)})")
-    apply(clarify) using neq_coreinit_rdsamp apply (simp add:E\<^sub>e_def)
-  using evtrgfset_def apply blast
-  apply(case_tac "ef1 \<in> (\<Union>(k, p).{(Schedule k p, Schedule_RGCond k p)})")
-   apply(case_tac "ef2 \<in> (\<Union>k. {(Core_Init k, Core_Init_RGCond k)})")
-    apply(clarify) using neq_coreinit_sched apply (metis E\<^sub>e_def fst_conv)
-  apply(case_tac "ef2 \<in> (\<Union>(k, p).{(Schedule k p, Schedule_RGCond k p)})")
-  apply(clarify) using neq_schedule apply (metis E\<^sub>e_def fst_conv)
-  apply(case_tac "ef2 \<in> (\<Union>(k, p, m).{(Send_Que_Message k p m, Send_Que_Message_RGCond k p m)})")
-  apply(clarify) using neq_sched_wrtsamp apply (simp add: E\<^sub>e_def)
-  apply(case_tac "ef2 \<in> (\<Union>(k, p).{(Recv_Que_Message k p, Recv_Que_Message_RGCond k p)})")
-  apply(clarify) using neq_sched_rdsamp apply (simp add: E\<^sub>e_def)
-   apply(simp add: evtrgfset_def)
-  apply(case_tac "ef1 \<in> (\<Union>(k, p, m).{(Send_Que_Message k p m, Send_Que_Message_RGCond k p m)})")
-   apply(case_tac "ef2 \<in> (\<Union>k. {(Core_Init k, Core_Init_RGCond k)})")
-    apply(clarify) using neq_coreinit_wrtsamp apply (metis (no_types, opaque_lifting) E\<^sub>e_def prod.sel(1))
-   apply(case_tac "ef2 \<in> (\<Union>(k, p).{(Schedule k p, Schedule_RGCond k p)})")
-    apply(clarify) using neq_sched_wrtsamp apply (metis (no_types, opaque_lifting) E\<^sub>e_def prod.sel(1))
-   apply(case_tac "ef2 \<in> (\<Union>(k, p, m).{(Send_Que_Message k p m, Send_Que_Message_RGCond k p m)})")
-    apply(clarify) using neq_wrt_samp apply (metis (no_types, opaque_lifting) E\<^sub>e_def prod.sel(1))
-   apply(case_tac "ef2 \<in> (\<Union>(k, p).{(Recv_Que_Message k p, Recv_Que_Message_RGCond k p)})")
-    apply(clarify) using neq_wrtsamp_rdsamp apply (metis (no_types, opaque_lifting) E\<^sub>e_def prod.sel(1))
-   apply(simp add: evtrgfset_def)
-  apply(case_tac "ef1 \<in> (\<Union>(k, p).{(Recv_Que_Message k p, Recv_Que_Message_RGCond k p)})")
-   apply(case_tac "ef2 \<in> (\<Union>k. {(Core_Init k, Core_Init_RGCond k)})")
-    apply(clarify) using neq_coreinit_rdsamp apply (metis (no_types, opaque_lifting) E\<^sub>e_def prod.sel(1))
-   apply(case_tac "ef2 \<in> (\<Union>(k, p).{(Schedule k p, Schedule_RGCond k p)})")
-    apply(clarify) using neq_sched_rdsamp apply (metis (no_types, opaque_lifting) E\<^sub>e_def prod.sel(1))
-   apply(case_tac "ef2 \<in> (\<Union>(k, p, m).{(Send_Que_Message k p m, Send_Que_Message_RGCond k p m)})")
-  apply(clarify) using neq_wrtsamp_rdsamp apply (metis (no_types, opaque_lifting) E\<^sub>e_def prod.sel(1))
-  apply(case_tac "ef2 \<in> (\<Union>(k, p).{(Recv_Que_Message k p, Recv_Que_Message_RGCond k p)})")
-    apply(clarify) using neq_rd_samp apply (metis (no_types, opaque_lifting) E\<^sub>e_def prod.sel(1))
-  by(simp add: evtrgfset_def)+
+lemma obs_cap_equiva : "\<lbrakk>\<forall>c. p2p conf (chdest conf c) = x1 \<longrightarrow> qbufsize\<^sub>a s1 c = qbufsize\<^sub>a s2 c\<rbrakk> 
+                        \<Longrightarrow>  obs_cap_part\<^sub>a s2 x1 = obs_cap_part\<^sub>a s1 x1"
+  apply (simp add: obs_cap_part\<^sub>a_def)
+  by force
 
-lemma evtrgfset_func: "\<forall>ef\<in>evtrgfset. evtrgffun (E\<^sub>e ef) = Some (snd ef)" 
-  proof -
-  {
-    fix ef
-    assume a0: "ef\<in>evtrgfset"
-    then have "E\<^sub>e ef\<in>Domain evtrgfset" by (metis Domain_iff E\<^sub>e_def surjective_pairing) 
-    then obtain ef1 where a1: "ef1\<in>evtrgfset \<and> E\<^sub>e ef1 = E\<^sub>e ef \<and> evtrgffun (E\<^sub>e ef) = Some (snd ef1)" 
-      using evtrgffun_exist[rule_format,of "E\<^sub>e ef"] by auto
-    have "evtrgffun (E\<^sub>e ef) = Some (snd ef)"
-      proof(cases "ef1 = ef")
-        assume "ef1 = ef"
-        with a1 show ?thesis by simp
-      next
-        assume b0: "ef1\<noteq>ef"
-        with diff_e_in_evtrgfset a0 a1 have "E\<^sub>e ef1 \<noteq> E\<^sub>e ef" by blast
-        with a1 show ?thesis by simp
-      qed
-  }
-  then show ?thesis by auto
-qed
+definition state_obs_part\<^sub>a :: "State\<^sub>a \<Rightarrow> Part \<Rightarrow> State\<^sub>a"
+  where "state_obs_part\<^sub>a s p \<equiv> s0\<^sub>a\<lparr>partst\<^sub>a := (partst\<^sub>a s0\<^sub>a) (p := (partst\<^sub>a s) p), 
+                                  qbufsize\<^sub>a := obs_cap_part\<^sub>a s p\<rparr>"
 
-lemma all_basic_evts_arinc_help: "\<forall>k. ef\<in>all_evts_es (fst (ARINCXKernel_Spec k)) \<longrightarrow> is_basicevt (E\<^sub>e ef)"
-  proof -
-  {
-    fix k
-    assume p0: "ef\<in>all_evts_es (fst (ARINCXKernel_Spec k))" 
-    then have "ef\<in>all_evts_es (fst (EvtSys_on_Core_RGF k))" by (simp add:ARINCXKernel_Spec_def)
-    then have "ef\<in>insert (Core_Init_RGF k) (all_evts_es (fst (EvtSys1_on_Core_RGF k)))" 
-      by (simp add:EvtSys_on_Core_RGF_def)
-    then have "ef = (Core_Init_RGF k) \<or> ef\<in>all_evts_es (fst (EvtSys1_on_Core_RGF k))" by auto
-    then have "is_basicevt (E\<^sub>e ef)"
-      proof
-        assume a0: "ef = Core_Init_RGF k"
-        then show ?thesis 
-          using Core_Init_RGF_def Core_Init_def by (simp add: E\<^sub>e_def)
-      next
-        assume a1: "ef\<in>all_evts_es (fst (EvtSys1_on_Core_RGF k))"
-        then have "ef\<in>{ef. \<exists>p. ef = Schedule_RGF k p} \<union>
-                      {ef. \<exists>p m. ef = Send_Que_Message_RGF k p m} \<union>
-                      {ef. \<exists>p. ef = Recv_Que_Message_RGF k p}" 
-          using all_evts_es_esys EvtSys1_on_Core_RGF_def by auto
-        then have "ef\<in>{ef. \<exists>p. ef = Schedule_RGF k p} 
-                  \<or> ef\<in>{ef. \<exists>p m. ef = Send_Que_Message_RGF k p m} 
-                  \<or> ef\<in>{ef. \<exists>p. ef = Recv_Que_Message_RGF k p}" by auto
-        then show ?thesis
-          proof
-            assume "ef\<in>{ef. \<exists>p. ef = Schedule_RGF k p}"
-            then have  "\<exists>p. ef = Schedule_RGF k p" by auto
-            then obtain p where "ef = Schedule_RGF k p" by auto
-            then show ?thesis by (simp add: E\<^sub>e_def Schedule_RGF_def Schedule_def)
-          next
-            assume "ef\<in>{ef. \<exists>p m. ef = Send_Que_Message_RGF k p m}
-                    \<or> ef\<in>{ef. \<exists>p. ef = Recv_Que_Message_RGF k p}"
-            then show ?thesis 
-              proof
-                assume "ef\<in>{ef. \<exists>p m. ef = Send_Que_Message_RGF k p m}"
-                then have "\<exists>p m. ef = Send_Que_Message_RGF k p m" by auto
-                then obtain p and m where "ef = Send_Que_Message_RGF k p m" by auto
-                then show ?thesis by (simp add: E\<^sub>e_def Send_Que_Message_RGF_def Send_Que_Message_def)
-              next
-                assume "ef\<in>{ef. \<exists>p. ef = Recv_Que_Message_RGF k p}"
-                then have "\<exists>p. ef = Recv_Que_Message_RGF k p" by auto
-                then obtain p where "ef = Recv_Que_Message_RGF k p" by auto
-                then show ?thesis by (simp add: E\<^sub>e_def Recv_Que_Message_RGF_def Recv_Que_Message_def) 
-              qed
-          qed
-      qed
-  }
-  then show ?thesis by auto
-  qed
+primrec state_obs\<^sub>a :: "State\<^sub>a \<Rightarrow> Domain \<Rightarrow> State\<^sub>a"
+  where "state_obs\<^sub>a s (P p) = state_obs_part\<^sub>a s p" |
+        "state_obs\<^sub>a s (S p) = state_obs_sched\<^sub>a s p"|
+        "state_obs\<^sub>a s F = s0\<^sub>a"
 
-lemma all_basic_evts_arinc: "\<forall>ef\<in>all_evts ARINCXKernel_Spec. is_basicevt (E\<^sub>e ef)" 
-  using all_evts_def[of ARINCXKernel_Spec] all_basic_evts_arinc_help by auto
+definition state_equiv\<^sub>a :: "State\<^sub>a \<Rightarrow> Domain \<Rightarrow> State\<^sub>a \<Rightarrow> bool" ("(_ \<sim>\<^sub>a_\<sim>\<^sub>a _)" [70,69,70] 60)
+  where "state_equiv\<^sub>a s d t \<equiv> state_obs\<^sub>a s d = state_obs\<^sub>a t d"
 
-lemma bsc_evts_rgfs: "\<forall>erg\<in>all_evts (ARINCXKernel_Spec). (evtrgffun (E\<^sub>e erg))  = Some (snd erg)"
-  using evtrgfset_func evtrgfset_eq_allevts_ARINCSpec by simp
+lemma state_equiv_transitivea: "\<lbrakk>s \<sim>\<^sub>a d \<sim>\<^sub>a t; t \<sim>\<^sub>a d \<sim>\<^sub>a r\<rbrakk> \<Longrightarrow> s \<sim>\<^sub>a d \<sim>\<^sub>a r"
+  by (simp add:state_equiv\<^sub>a_def)
+    
+lemma state_equiv_symmetrica : "s \<sim>\<^sub>a d \<sim>\<^sub>a t \<Longrightarrow> t \<sim>\<^sub>a d \<sim>\<^sub>a s"
+  by (simp add:state_equiv\<^sub>a_def)
+
+lemma state_equiv_reflexivea : "s \<sim>\<^sub>a d \<sim>\<^sub>a s"
+  by (simp add:state_equiv\<^sub>a_def)
+
+subsection \<open>Simulation Relation\<close>
+
+definition state_inv :: " (State\<^sub>c \<times> State\<^sub>a) set" 
+  where "state_inv = {(s\<^sub>c, s\<^sub>a). cur\<^sub>c s\<^sub>c = cur\<^sub>a s\<^sub>a \<and> partst\<^sub>c s\<^sub>c = partst\<^sub>a s\<^sub>a \<and> obsize\<^sub>c s\<^sub>c = qbufsize\<^sub>a s\<^sub>a
+         \<and> (\<forall>q. qlock\<^sub>c s\<^sub>c q = None \<longrightarrow> obsize\<^sub>c s\<^sub>c q = qbufsize\<^sub>c s\<^sub>c q)}"
+
+definition event_map :: "(EventLabel, Core, State\<^sub>c, Prog\<^sub>c) event \<Rightarrow> (EventLabel, Core, State\<^sub>a, Prog\<^sub>a) event"
+  where "event_map a = "
+
+subsection \<open>Rely-guarantee condition of programs\<close>
 
 
-interpretation PiCore_RG_IFS ptranI petranI None cpts_pI cpts_of_pI prog_validityI ann_preserves_p
-                            assume_pI commit_pI preserves_p rghoare_pI interf state_equiv domevt \<Gamma>
-                            C0 "exec_step \<Gamma>" state_obs ARINCXKernel_Spec s0 x0 evtrgffun 
-                            "paresys_spec ARINCXKernel_Spec"
-proof
-  show "\<forall>a b c u. a \<sim>u\<sim> b \<and> b \<sim>u\<sim> c \<longrightarrow> a \<sim>u\<sim> c"
-    using state_equiv_transitive by blast
-  show "\<forall>a b u. a \<sim>u\<sim> b \<longrightarrow> b \<sim>u\<sim> a"
-    using state_equiv_symmetric by blast
-  show "\<forall>a u. a \<sim>u\<sim> a"
-    by (simp add: state_equiv_reflexive)
-  show "C0 = (paresys_spec ARINCXKernel_Spec, s0, x0)"
-    using C0_init by blast
-  show "paresys_spec ARINCXKernel_Spec = paresys_spec ARINCXKernel_Spec" by simp
-  show "\<forall>ef\<in>all_evts ARINCXKernel_Spec. is_basicevt (E\<^sub>e ef)" 
-    using all_basic_evts_arinc by blast
-  show "\<forall>k. \<Gamma> \<turnstile> fst (ARINCXKernel_Spec k) sat\<^sub>s [Pre\<^sub>e\<^sub>s (ARINCXKernel_Spec k), Rely\<^sub>e\<^sub>s (ARINCXKernel_Spec k), 
-            Guar\<^sub>e\<^sub>s (ARINCXKernel_Spec k), Post\<^sub>e\<^sub>s (ARINCXKernel_Spec k)]"
-    by (simp add: spec_sat_rg)
-  show "\<forall>k. s0 \<in> Pre\<^sub>e\<^sub>s (ARINCXKernel_Spec k)"
-    using spec_sat_init by fastforce
-  show " \<forall>k j. j \<noteq> k \<longrightarrow> Guar\<^sub>e\<^sub>s (ARINCXKernel_Spec j) \<subseteq> Rely\<^sub>e\<^sub>s (ARINCXKernel_Spec k)"
-    using spec_rg_com by blast
-  show "\<forall>erg\<in>all_evts ARINCXKernel_Spec. the (evtrgffun (E\<^sub>e erg)) = snd erg"
-    using bsc_evts_rgfs by fastforce
-  show "\<And>a. exec_step \<Gamma> a \<equiv> {(P, Q). \<Gamma> \<turnstile> P -pes-actk a\<rightarrow> Q \<and>
-        ((\<exists>e k. actk a = EvtEnt e\<sharp>k \<and> eventof a = e \<and> domevt (gets P) e = domain a) \<or>
-        (\<exists>c k. actk a = Cmd c\<sharp>k \<and> eventof a = getx P k \<and> domevt (gets P) (eventof a) = domain a))}"
-    by (simp add: exec_step_def)
-qed
+abbreviation "init\<^sub>c_rely k \<equiv> \<lbrace>(\<forall>p. p2s conf p = c2s conf k \<longrightarrow> \<ordfeminine>partst\<^sub>c p = \<ordmasculine>partst\<^sub>c p)\<rbrace> \<union> Id"
+abbreviation "init\<^sub>c_guar k \<equiv> \<lbrace>\<ordfeminine>cur\<^sub>c = \<ordmasculine>cur\<^sub>c \<and> \<ordfeminine>qbuf\<^sub>c = \<ordmasculine>qbuf\<^sub>c \<and> \<ordfeminine>qbufsize\<^sub>c = \<ordmasculine>qbufsize\<^sub>c
+            \<and> \<ordfeminine>qlock\<^sub>c = \<ordmasculine>qlock\<^sub>c \<and> \<ordfeminine>obsize\<^sub>c = \<ordmasculine>obsize\<^sub>c  
+            \<and> (\<forall>p. p2s conf p = c2s conf k \<longrightarrow> \<ordmasculine>partst\<^sub>c p = IDLE \<and> \<ordfeminine>partst\<^sub>c p = READY)
+            \<and> (\<forall>p. p2s conf p \<noteq> c2s conf k \<longrightarrow> \<ordfeminine>partst\<^sub>c p = \<ordmasculine>partst\<^sub>c p)\<rbrace> \<union> Id"
+
+definition init_map :: "Core \<Rightarrow> State\<^sub>c com \<rightharpoonup> State\<^sub>a com"
+  where "init_map k = 
+        [ \<acute>partst\<^sub>c := (\<lambda>p. if p2s conf p = c2s conf k \<and> \<acute>partst\<^sub>c p = IDLE then READY else \<acute>partst\<^sub>c p)
+       \<mapsto> \<acute>partst\<^sub>a := (\<lambda>p. if p2s conf p = c2s conf k \<and> \<acute>partst\<^sub>a p = IDLE then READY else \<acute>partst\<^sub>a p)]"
+
+definition init_pre :: "Core \<Rightarrow> (State\<^sub>c \<times> State\<^sub>a) set"
+  where "init_pre k = state_inv \<inter> {(s\<^sub>c, s\<^sub>a). (\<forall>p. p2s conf p = c2s conf k \<longrightarrow> partst\<^sub>c s\<^sub>c p = IDLE)}"
+abbreviation "init_post \<equiv> state_inv"
 
 
-subsection \<open>Proof of Events satisfy the UCs \<close>
+abbreviation "init\<^sub>a_rely k \<equiv> UNIV"
+abbreviation "init\<^sub>a_guar k \<equiv> UNIV"
 
+lemma init_sim : "prog_sim_pre 
+      (Some (\<acute>partst\<^sub>c := (\<lambda>p. if p2s conf p = c2s conf k \<and> \<acute>partst\<^sub>c p = IDLE then READY else \<acute>partst\<^sub>c p)))
+      (init\<^sub>c_rely k) (init\<^sub>c_guar k) 
+      state_inv (init_map k) (init_pre k) init_post
+      (Some (\<acute>partst\<^sub>a := (\<lambda>p. if p2s conf p = c2s conf k \<and> \<acute>partst\<^sub>a p = IDLE then READY else \<acute>partst\<^sub>a p)))
+      (init\<^sub>a_rely k) (init\<^sub>a_guar k)"
+  apply (rule Basic_Sound, simp_all add: init_pre_def init_map_def)
+  apply (simp add: stable_alpha)
+   apply (rule stable_conj, simp add: stable_alpha)
+   apply (simp add: Stable_def related_transitions_def)
+  apply blast
+  apply clarify
+  apply (simp add: state_inv_def)
+  by force
 
-interpretation Anno_SIMP_IFS interf state_equiv domevt
-  by (simp add: Anno_SIMP_IFS_def state_equiv_def)
+abbreviation "schedule\<^sub>c_rely k p \<equiv> \<lbrace>\<ordfeminine>cur\<^sub>c (c2s conf k) = \<ordmasculine>cur\<^sub>c (c2s conf k) \<and>
+                                   (\<forall>p. p2s conf p = c2s conf k \<longrightarrow> \<ordfeminine>partst\<^sub>c p = \<ordmasculine>partst\<^sub>c p)\<rbrace> \<union> Id"
 
+abbreviation "schedule\<^sub>c_guar k p \<equiv> \<lbrace>\<ordfeminine>qbuf\<^sub>c = \<ordmasculine>qbuf\<^sub>c \<and> \<ordfeminine>qbufsize\<^sub>c = \<ordmasculine>qbufsize\<^sub>c \<and> \<ordfeminine>qlock\<^sub>c = \<ordmasculine>qlock\<^sub>c 
+      \<and> \<ordfeminine>obsize\<^sub>c = \<ordmasculine>obsize\<^sub>c \<and> (\<forall>c. c \<noteq> k \<longrightarrow> \<ordfeminine>cur\<^sub>c (c2s conf c) = \<ordmasculine>cur\<^sub>c (c2s conf c))
+      \<and> (\<forall>p. p2s conf p \<noteq> c2s conf k \<longrightarrow> \<ordfeminine>partst\<^sub>c p = \<ordmasculine>partst\<^sub>c p)\<rbrace> \<union> Id"
 
-lemma s0_update_help: "\<lbrakk>partst1 = partst2; qbufsize1 = qbufsize2 \<rbrakk> \<Longrightarrow> 
-                      s0\<lparr> partst := partst1, qbufsize := qbufsize1 \<rparr> = s0\<lparr> partst := partst2, qbufsize := qbufsize2\<rparr>"
-  by blast
+definition schedule_map :: "Core \<Rightarrow> Part \<Rightarrow> State\<^sub>c com \<rightharpoonup> State\<^sub>a com"
+  where "schedule_map k p = 
+        [ATOMIC
+           IF (\<acute>cur\<^sub>c((c2s conf) k) \<noteq> None) THEN    
+             \<acute>partst\<^sub>c := \<acute>partst\<^sub>c(the (\<acute>cur\<^sub>c ((c2s conf) k)) := READY);;
+             \<acute>cur\<^sub>c := \<acute>cur\<^sub>c((c2s conf) k := None)
+           FI;;
+           \<acute>cur\<^sub>c := \<acute>cur\<^sub>c((c2s conf k) := Some p);;
+           \<acute>partst\<^sub>c := \<acute>partst\<^sub>c(p := RUN)
+         END
+      \<mapsto> ATOMIC
+           IF (\<acute>cur\<^sub>a((c2s conf) k) \<noteq> None) THEN    
+             \<acute>partst\<^sub>a := \<acute>partst\<^sub>a(the (\<acute>cur\<^sub>a ((c2s conf) k)) := READY)
+           FI;;
+           \<acute>cur\<^sub>a := \<acute>cur\<^sub>a((c2s conf k) := Some p);;
+           \<acute>partst\<^sub>a := \<acute>partst\<^sub>a(p := RUN)
+         END]"
 
-lemma Core_Init_sat_LRE: 
-  "\<forall>u s1 s2 x. (s1,s2) \<in> Guar\<^sub>f (Core_Init_RGCond x)
-                \<longrightarrow> ((domevt s1 (Core_Init x)) \<setminus>\<leadsto> u \<longrightarrow> s1 \<sim>u\<sim> s2)"
-  apply (simp add: Core_Init_RGCond_def Guar\<^sub>f_def getrgformula_def, clarsimp)
-  apply (simp add: domevt_def get_evt_core_def Core_Init_def label_def get_evt_el_def get_evt_label_def)
-  apply (case_tac u, clarify)
-    apply (case_tac "p2s conf x1 = c2s conf x")
-     apply (simp add: interf_def)
-    apply (simp add: state_equiv_def state_obs_part_def, clarify)
-     apply (rule s0_update_help)
-      apply (simp add: interf_def noninterf_def)
-  using obs_cap_equiv apply presburger
-    apply (smt (verit) State.fold_congs(3) State.update_convs(4) System_Init_def bij_c2s 
-    bij_pointE fst_conv obs_cap_equiv1 s0_init state_equiv_def state_obs.simps(1) state_obs_part_def)
-  using state_equiv_def state_obs.simps(2) state_obs_sched_def apply presburger
-  by (simp add: state_equiv_def)
+abbreviation "schedule_pre1 k \<equiv> {(s\<^sub>c, s\<^sub>a). 
+  ((cur\<^sub>c s\<^sub>c) (c2s conf k) \<noteq> None \<longrightarrow> p2s conf (the ((cur\<^sub>c s\<^sub>c) (c2s conf k))) = c2s conf k) \<and>
+  ((cur\<^sub>a s\<^sub>a) (c2s conf k) \<noteq> None \<longrightarrow> p2s conf (the ((cur\<^sub>a s\<^sub>a) (c2s conf k))) = c2s conf k)}"
 
+abbreviation "schdule_pre k p \<equiv> state_inv \<inter> \<lbrace>p2s conf p = c2s conf k\<rbrace> \<inter> schedule_pre1 k"
+abbreviation "schdule_post \<equiv> state_inv"
 
-lemma Schedule_sat_LRE: 
-  "\<forall>u s1 s2 x p. (s1,s2) \<in> Guar\<^sub>f (Schedule_RGCond x p) 
-                \<longrightarrow> ((domevt s1 (Schedule x p)) \<setminus>\<leadsto> u \<longrightarrow> s1 \<sim>u\<sim> s2)"
-  apply (simp add: Schedule_RGCond_def Guar\<^sub>f_def getrgformula_def, clarsimp)
-  apply (simp add: domevt_def get_evt_core_def Schedule_def label_def get_evt_el_def get_evt_label_def)
-  apply (case_tac u)
-    apply (simp add: state_equiv_def state_obs_part_def, clarsimp)
-    apply (rule s0_update_help)
-     apply (case_tac "p2s conf x1 = c2s conf x")
-      apply (simp add: interf_def noninterf_def)
-     apply presburger
-  using obs_cap_part_def apply presburger
-   apply (simp add: state_equiv_def state_obs_sched_def)
-   apply (metis fun_upd_other interf_def noninterf_def)
-  using state_equiv_def by auto[1]
-
-
-lemma ch_chonn_help1 : "\<lbrakk>port_of_part conf p y; c = ch_srcqport conf p; is_src_qport conf p; y \<noteq> p2p conf (chdest conf c)\<rbrakk> 
-   \<Longrightarrow> ch_conn conf y (p2p conf (chdest conf c))"
-  apply (simp add: ch_conn_def, rule_tac x = c in exI)
-  apply (simp add: port_of_part_def is_src_qport_def image_def ch_srcqport_def)
-  by (metis (mono_tags, lifting) someI2)
-
-lemma ch_chonn_help2 : "\<lbrakk>port_of_part conf p y; is_src_qport conf p; y \<noteq> p2p conf (chdest conf c); P y \<setminus>\<leadsto> P (p2p conf (chdest conf c))\<rbrakk>
-          \<Longrightarrow> c \<noteq> ch_srcqport conf p"
-  using ch_chonn_help1 interf_def noninterf_def by fastforce
-
-lemma Send_Que_sat_LRE:
-  "\<forall>u s1 s2 k. (s1,s2) \<in> Guar\<^sub>f (Send_Que_Message_RGCond x p m) 
-                \<longrightarrow> ((domevt s1 (Send_Que_Message x p m)) \<setminus>\<leadsto> u \<longrightarrow> s1 \<sim>u\<sim> s2)"
-  apply (simp add: Send_Que_Message_RGCond_def Guar\<^sub>f_def getrgformula_def, clarsimp)
-  apply (simp add: domevt_def get_evt_core_def Send_Que_Message_def label_def get_evt_el_def get_evt_label_def)
-  apply (case_tac "(cur s1) (c2s conf x) = None")
-  apply (metis State.surjective old.unit.exhaust state_equiv_def)
-  apply (case_tac u, clarsimp)
-    apply (case_tac "is_src_qport conf p \<and> port_of_part conf p y", simp)
-     apply (metis ch_chonn_help2 interf_def noninterf_def obs_cap_equiv state_equiv_def state_obs.simps(1) state_obs_part_def)
-    apply (simp add: state_equiv_def state_obs_def)
-    apply (metis State.surjective old.unit.exhaust)
-   apply (simp add: state_equiv_def state_obs_sched_def)
-  using state_equiv_def state_obs.simps(3) by presburger
-
-lemma Recv_Que_sat_LRE:
-  "\<forall>u s1 s2 k. (s1,s2) \<in> Guar\<^sub>f (Recv_Que_Message_RGCond x p) 
-                \<longrightarrow> ((domevt s1 (Recv_Que_Message x p)) \<setminus>\<leadsto> u \<longrightarrow> s1 \<sim>u\<sim> s2)"
-  apply (simp add: Recv_Que_Message_RGCond_def Guar\<^sub>f_def getrgformula_def, clarsimp)
-  apply (simp add: domevt_def get_evt_core_def Recv_Que_Message_def label_def get_evt_el_def get_evt_label_def)
-  apply (case_tac "(cur s1) (c2s conf x) = None")
-  apply (metis (mono_tags, lifting) State.surjective old.unit.exhaust state_equiv_def)
-  apply (case_tac u)
-    apply (case_tac "x1 = the ((cur s1) (c2s conf x))")
-  using interf_def noninterf_def apply force
-    apply (simp add: state_equiv_def  state_obs_part_def)
-    apply (rule s0_update_help)
-     apply blast
-    apply (rule obs_cap_equiv, clarsimp)
-    apply (case_tac "is_dest_qport conf p \<and> port_of_part conf p y", simp)
-     apply (drule_tac a = c in all_impD)
-      apply (simp add: ch_destqport_def is_dest_qport_def port_of_part_def image_def)
-      apply (metis (mono_tags, lifting)  someI)
-     apply blast
-    apply presburger
-   apply (simp add: state_equiv_def state_obs_sched_def)
-  using state_equiv_def state_obs.simps(3) by presburger
-
-
-lemma uwce_LRE_help: "\<forall>x. ef \<in> all_evts_es (fst (ARINCXKernel_Spec x)) \<and> (s1,s2) \<in> Guar\<^sub>e ef \<longrightarrow> 
-                                    ((domevt s1 (E\<^sub>e ef)) \<setminus>\<leadsto> u \<longrightarrow> s1 \<sim>u\<sim> s2)"
-  proof -
-  {
-    fix x
-    assume p0: "ef\<in>all_evts_es (fst (ARINCXKernel_Spec x))" 
-    then have "ef\<in>all_evts_es (fst (EvtSys_on_Core_RGF x))" by (simp add:ARINCXKernel_Spec_def)
-    then have "ef\<in>insert (Core_Init_RGF x) (all_evts_es (fst (EvtSys1_on_Core_RGF x)))" 
-      by (simp add:EvtSys_on_Core_RGF_def)
-    then have "ef = (Core_Init_RGF x) \<or> ef\<in>all_evts_es (fst (EvtSys1_on_Core_RGF x))" by auto
-    then have "(s1,s2) \<in> Guar\<^sub>e ef \<longrightarrow> ((domevt s1 (E\<^sub>e ef)) \<setminus>\<leadsto> u \<longrightarrow> s1 \<sim>u\<sim> s2)"
-      proof
-        assume a0: "ef = Core_Init_RGF x"
-        then show ?thesis
-          by (simp add: Core_Init_RGF_def Core_Init_sat_LRE E\<^sub>e_def Guar\<^sub>e_def Guar\<^sub>f_def)          
-      next
-        assume a1: "ef\<in>all_evts_es (fst (EvtSys1_on_Core_RGF x))"
-        then have "ef\<in>{ef. \<exists>p. ef = Schedule_RGF x p} \<union>
-                      {ef. \<exists>p m. ef = Send_Que_Message_RGF x p m} \<union>
-                      {ef. \<exists>p. ef = Recv_Que_Message_RGF x p}" 
-          using all_evts_es_esys EvtSys1_on_Core_RGF_def by auto
-        then have "ef\<in>{ef. \<exists>p. ef = Schedule_RGF x p} 
-                  \<or> ef\<in>{ef. \<exists>p m. ef = Send_Que_Message_RGF x p m} 
-                  \<or> ef\<in>{ef. \<exists>p. ef = Recv_Que_Message_RGF x p}" by auto
-        then show ?thesis
-          proof
-            assume "ef\<in>{ef. \<exists>p. ef = Schedule_RGF x p}"
-            then have "\<exists>p. ef = Schedule_RGF x p" by auto
-            then obtain p where "ef = Schedule_RGF x p" by auto
-            then show ?thesis 
-              by (simp add: E\<^sub>e_def Guar\<^sub>e_def Guar\<^sub>f_def Schedule_RGF_def Schedule_sat_LRE) 
-          next
-            assume "ef\<in>{ef. \<exists>p m. ef = Send_Que_Message_RGF x p m}
-                    \<or> ef\<in>{ef. \<exists>p. ef = Recv_Que_Message_RGF x p}"
-            then show ?thesis 
-              proof
-                assume "ef\<in>{ef. \<exists>p m. ef = Send_Que_Message_RGF x p m}"
-                then have "\<exists>p m. ef = Send_Que_Message_RGF x p m" by auto
-                then obtain p and m where "ef = Send_Que_Message_RGF x p m" by auto
-                then show ?thesis 
-                  by (simp add: E\<^sub>e_def Guar\<^sub>e_def Guar\<^sub>f_def Send_Que_Message_RGF_def Send_Que_sat_LRE)
-              next
-                assume "ef\<in>{ef. \<exists>p. ef = Recv_Que_Message_RGF x p}"
-                then have "\<exists>p. ef = Recv_Que_Message_RGF x p" by auto
-                then obtain p where "ef = Recv_Que_Message_RGF x p" by auto
-                then show ?thesis 
-                  by (simp add: E\<^sub>e_def Guar\<^sub>e_def Guar\<^sub>f_def Recv_Que_Message_RGF_def Recv_Que_sat_LRE)
-              qed
-          qed
-      qed
-  }
-  then show ?thesis by auto
-qed
+abbreviation "schedule\<^sub>a_rely \<equiv> UNIV"
+abbreviation "schedule\<^sub>a_guar \<equiv> UNIV"
 
 
 
-lemma Core_Init_sat_SCE: "sc_p_sat (the (body_e (Core_Init k))) (Core_Init k)"
-  apply (simp add: body_e_def Core_Init_def body_def sc_p_sat.Basic)
-  apply (rule sc_p_sat.Basic, clarsimp)
-  apply (case_tac u)
-    apply (simp add: state_equiv_def state_obs_part_def)
-    apply (simp add: System_Init_def s0_init)
-    apply (metis (no_types, lifting) State.select_convs(3) State.surjective  State.update_convs(4) obs_cap_equiv1)
-  using state_equiv_def state_obs_sched_def apply auto[1]
-  using state_equiv_def state_obs.simps(3) apply presburger
-  done
+abbreviation "sched_await_mid1\<^sub>c s k p \<equiv> 
+    {s'. ((cur\<^sub>c s) (c2s conf k) = None \<longrightarrow> s' = s \<lparr>cur\<^sub>c := (cur\<^sub>c s) ((c2s conf k) := Some p)\<rparr>) \<and> 
+         ((cur\<^sub>c s) (c2s conf k) \<noteq> None \<longrightarrow> s' = s \<lparr>cur\<^sub>c := (cur\<^sub>c s) ((c2s conf k) := Some p),
+                   partst\<^sub>c := (partst\<^sub>c s) (the ((cur\<^sub>c s) (c2s conf k)) := READY)\<rparr>)}"
 
-lemma Schedule_sat_SCE_h1: " 
-        \<turnstile>\<^sub>I Some (\<lbrace>True \<rbrace>\<acute>partst := \<acute>partst(the (\<acute>cur (c2s conf k)) := READY);;
-         \<lbrace>True \<rbrace> \<acute>cur := \<acute>cur (c2s conf k := None)) sat\<^sub>p 
-        [\<lbrace>p2s conf p = c2s conf k \<and> p2s conf (the (\<acute>cur (c2s conf k))) = c2s conf k\<rbrace> \<inter> {V}, 
-         {(s, t). s = t}, UNIV, \<lbrace>\<acute>qbuf = qbuf V \<and> \<acute>qbufsize = qbufsize V \<and> \<acute>cur = (cur V)(c2s conf k := None) 
-        \<and> \<acute>partst = (partst V)(the (cur V (c2s conf k)) := READY) \<and> (\<forall>p. p2s conf p \<noteq> c2s conf k \<longrightarrow> \<acute>partst p = partst V p)\<rbrace>]"
-  apply (case_tac "p2s conf p = c2s conf k \<and> p2s conf (the ((cur V) (c2s conf k))) = c2s conf k ")
-   apply simp
-   apply(rule rghoare_p.Seq[where mid="{s. s = V \<lparr> partst := (partst V) (the ((cur V) (c2s conf k)) := READY)\<rparr>
-         \<and> p2s conf p = c2s conf k}"])
-    apply (rule rghoare_p.Basic, simp)
-       apply force
-      apply simp
-     apply (simp add: stable_def)+
-  apply (rule rghoare_p.Basic, simp, simp, simp)
-    apply (simp add: stable_def, simp add: stable_def)
-  apply(rule rghoare_p.Seq[where mid="{}"])
-   apply (rule rghoare_p.Basic)
+abbreviation "sched_await_mid2\<^sub>c s k  \<equiv> 
+    {s'. ((cur\<^sub>c s) (c2s conf k) = None \<longrightarrow> s' = s) \<and> 
+         ((cur\<^sub>c s) (c2s conf k) \<noteq> None \<longrightarrow> s' = s \<lparr>cur\<^sub>c := (cur\<^sub>c s) ((c2s conf k) := None),
+                   partst\<^sub>c := (partst\<^sub>c s) (the ((cur\<^sub>c s) (c2s conf k)) := READY)\<rparr>)}"
+
+abbreviation "sched_await_if_mid\<^sub>c s k  \<equiv> 
+    {s'. (cur\<^sub>c s) (c2s conf k) \<noteq> None \<and> s' = s \<lparr>partst\<^sub>c := (partst\<^sub>c s) (the ((cur\<^sub>c s) (c2s conf k)) := READY)\<rparr>}"
+
+abbreviation "sched_await_post\<^sub>c s k p \<equiv> 
+    {s'. ((cur\<^sub>c s) (c2s conf k) = None \<longrightarrow> s' = s \<lparr>cur\<^sub>c := (cur\<^sub>c s) ((c2s conf k) := Some p),
+                                                 partst\<^sub>c := (partst\<^sub>c s) (p := RUN)\<rparr>) \<and> 
+         ((cur\<^sub>c s) (c2s conf k) \<noteq> None \<longrightarrow> s' = s \<lparr>cur\<^sub>c := (cur\<^sub>c s) ((c2s conf k) := Some p),
+                   partst\<^sub>c := (partst\<^sub>c s) (the ((cur\<^sub>c s) (c2s conf k)) := READY, p:= RUN)\<rparr>)}"
+
+lemma schedc_await_sat_post: "\<lbrakk>p2s conf p = c2s conf k; 
+      (\<exists>y. cur\<^sub>c s\<^sub>c (c2s conf k) = Some y) \<longrightarrow> p2s conf (the (cur\<^sub>c s\<^sub>c (c2s conf k))) = c2s conf k\<rbrakk> \<Longrightarrow>
+      \<turnstile> Await UNIV
+          (IF \<exists>y. \<acute>cur\<^sub>c (c2s conf k) = Some y THEN 
+             \<acute>partst\<^sub>c := \<acute>partst\<^sub>c(the (\<acute>cur\<^sub>c (c2s conf k)) := READY);; 
+             \<acute>cur\<^sub>c := \<acute>cur\<^sub>c(c2s conf k := None) 
+           FI;;
+           \<acute>cur\<^sub>c := \<acute>cur\<^sub>c(c2s conf k \<mapsto> p);;
+           \<acute>partst\<^sub>c := \<acute>partst\<^sub>c (p := RUN))
+           sat [{s\<^sub>c}, Id, schedule\<^sub>c_guar k p, sched_await_post\<^sub>c s\<^sub>c k p]"
+  apply (rule Await, simp_all add: stable_def, clarify)
+  apply (case_tac "s\<^sub>c \<noteq> V")
+   apply (rule Seq[where mid = "{}"])
+  apply (rule Seq[where mid = "{}"])
+     apply (rule Cond, simp add: stable_def)
+       apply (rule Seq[where mid = "{}"])
+        apply (rule Basic, simp_all add: stable_def)
+      apply (rule Basic, simp_all add: stable_def)
+     apply (simp add: Skip_def, rule Basic, simp_all add: stable_def)
+    apply (rule Basic, simp_all add: stable_def)
+   apply (rule Basic, simp_all add: stable_def)
+  apply (rule Seq[where mid = "sched_await_mid1\<^sub>c s\<^sub>c k p"])
+   apply (rule Seq[where mid = "sched_await_mid2\<^sub>c s\<^sub>c k"])
+    apply (rule Cond, simp add: stable_def)
+      apply (rule Seq[where mid = "sched_await_if_mid\<^sub>c s\<^sub>c k"])
+       apply (rule Basic)
+          apply blast
        apply (simp add: stable_def)+
-  apply (rule rghoare_p.Basic, simp_all)
-   apply (simp add: stable_def)+
-  by force
-
-lemma Schedule_sat_SCE_h2: "\<turnstile>\<^sub>I Some (\<lbrace>True \<rbrace> \<acute>cur := \<acute>cur(c2s conf k \<mapsto> p) ;;
-                         \<lbrace>True \<rbrace> \<acute>partst := \<acute>partst (p := RUN))
-      sat\<^sub>p [\<lbrace>p2s conf p = c2s conf k \<and> \<acute>cur (c2s conf k) = None\<rbrace> \<inter>  {V}, {(s, t). s = t}, UNIV, 
-            \<lbrace>\<acute>qbuf = qbuf V \<and> \<acute>qbufsize = qbufsize V \<and> \<acute>cur = (cur V)(c2s conf k \<mapsto> p) \<and> 
-             \<acute>partst = (partst V)(the (\<acute>cur (c2s conf k)) := RUN) \<and> (\<forall>p. p2s conf p \<noteq> c2s conf k 
-             \<longrightarrow> \<acute>partst p = partst V p)\<rbrace>]"
-  apply(case_tac "p2s conf p = c2s conf k \<and> (cur V) (c2s conf k) = None", simp)
-   apply(rule rghoare_p.Seq[where mid="{s. s = V \<lparr> cur := (cur V) (c2s conf k := Some p)\<rparr>}"])
-    apply (rule rghoare_p.Basic)
-        apply (simp add: stable_def)+
-   apply (rule rghoare_p.Basic, simp, simp)
-  using inj_surj_c2s injI surj_def apply (simp add: inj_eq)
-    apply(simp add:stable_def)+
-  apply(rule rghoare_p.Seq[where mid="{}"])
-   apply (rule rghoare_p.Basic, simp)
-      apply(simp add:stable_def)+
-  apply (rule rghoare_p.Basic, simp)
+      apply (rule Basic)
+         apply auto[1]
+       apply (simp add: stable_def)+
+     apply (simp add: Skip_def, rule Basic)
+        apply auto[1]
      apply (simp add: stable_def)+
+   apply (rule Basic)
+      apply auto[1]
+      apply (metis State\<^sub>c.surjective State\<^sub>c.update_convs(1) State\<^sub>c.update_convs(6))
+    apply (simp add: stable_def)+
+  apply (rule Basic, clarsimp)
+     apply (case_tac "cur\<^sub>c s\<^sub>c (c2s conf k) = None", simp)
+      apply (meson inj_eq inj_surj_c2s)
+     apply (simp add: inj_eq inj_surj_c2s)
+  by (simp add: stable_def)+
+
+abbreviation "sched_await_mid1\<^sub>a s k p \<equiv> 
+    {s'. ((cur\<^sub>a s) (c2s conf k) = None \<longrightarrow> s' = s \<lparr>cur\<^sub>a := (cur\<^sub>a s) ((c2s conf k) := Some p)\<rparr>) \<and> 
+         ((cur\<^sub>a s) (c2s conf k) \<noteq> None \<longrightarrow> s' = s \<lparr>cur\<^sub>a := (cur\<^sub>a s) ((c2s conf k) := Some p),
+                   partst\<^sub>a := (partst\<^sub>a s) (the ((cur\<^sub>a s) (c2s conf k)) := READY)\<rparr>)}"
+
+abbreviation "sched_await_mid2\<^sub>a s k  \<equiv> 
+    {s'. ((cur\<^sub>a s) (c2s conf k) = None \<longrightarrow> s' = s) \<and> 
+         ((cur\<^sub>a s) (c2s conf k) \<noteq> None \<longrightarrow> s' = s \<lparr>
+          partst\<^sub>a := (partst\<^sub>a s) (the ((cur\<^sub>a s) (c2s conf k)) := READY)\<rparr>)}"
+
+abbreviation "sched_await_post\<^sub>a s k p \<equiv> 
+    {s'. ((cur\<^sub>a s) (c2s conf k) = None \<longrightarrow> s' = s \<lparr>cur\<^sub>a := (cur\<^sub>a s) ((c2s conf k) := Some p),
+                                                 partst\<^sub>a := (partst\<^sub>a s) (p := RUN)\<rparr>) \<and>
+         ((cur\<^sub>a s) (c2s conf k) \<noteq> None \<longrightarrow>s' = s \<lparr>cur\<^sub>a := (cur\<^sub>a s) ((c2s conf k) := Some p),
+                   partst\<^sub>a := (partst\<^sub>a s) (the ((cur\<^sub>a s) (c2s conf k)) := READY, p := RUN)\<rparr>)}"
+
+lemma scheda_await_sat_post: "\<lbrakk>p2s conf p = c2s conf k; 
+      (\<exists>y. cur\<^sub>a s\<^sub>a (c2s conf k) = Some y) \<longrightarrow> p2s conf (the (cur\<^sub>a s\<^sub>a (c2s conf k))) = c2s conf k\<rbrakk> \<Longrightarrow>
+      \<turnstile> Await UNIV 
+          (IF \<exists>y. \<acute>cur\<^sub>a (c2s conf k) = Some y THEN 
+            \<acute>partst\<^sub>a := \<acute>partst\<^sub>a(the (\<acute>cur\<^sub>a (c2s conf k)) := READY) 
+           FI;; 
+          \<acute>cur\<^sub>a := \<acute>cur\<^sub>a(c2s conf k \<mapsto> p);; 
+          \<acute>partst\<^sub>a := \<acute>partst\<^sub>a(p := RUN)) 
+          sat [{s\<^sub>a}, Id, schedule\<^sub>a_guar, sched_await_post\<^sub>a s\<^sub>a k p]"
+  apply (rule Await, simp_all add: stable_def, clarify)
+  apply (case_tac "s\<^sub>a \<noteq> V")
+   apply (rule Seq[where mid = "{}"])
+    apply (rule Seq[where mid = "{}"])
+     apply (rule Cond, simp add: stable_def)
+        apply (rule Basic, simp_all add: stable_def)
+     apply (simp add: Skip_def, rule Basic, simp_all add: stable_def)
+    apply (rule Basic, simp_all add: stable_def)
+   apply (rule Basic, simp_all add: stable_def)
+  apply (rule Seq[where mid = "sched_await_mid1\<^sub>a s\<^sub>a k p"])
+   apply (rule Seq[where mid = "sched_await_mid2\<^sub>a s\<^sub>a k"])
+    apply (rule Cond)
+       apply (simp add: stable_def)+
+      apply (rule Basic)
+         apply auto[1]
+        apply (simp add: stable_def)+
+     apply (simp add: Skip_def, rule Basic)
+        apply auto[1]
+       apply (simp add: stable_def)+
+   apply (rule Basic, case_tac "cur\<^sub>a s\<^sub>a (c2s conf k) = None", simp, clarsimp)
+     apply (simp add: stable_def)+
+  apply (rule Basic, case_tac "cur\<^sub>a s\<^sub>a (c2s conf k) = None", simp, clarsimp)
+  by (simp add: stable_def)+
+
+lemma schedule_not_stuck: "not_stuck UNIV 
+      (IF (\<acute>cur\<^sub>a((c2s conf) k) \<noteq> None) THEN    
+         \<acute>partst\<^sub>a := \<acute>partst\<^sub>a(the (\<acute>cur\<^sub>a ((c2s conf) k)) := READY)
+      FI;;
+     \<acute>cur\<^sub>a := \<acute>cur\<^sub>a((c2s conf k) := Some p);;
+     \<acute>partst\<^sub>a := \<acute>partst\<^sub>a(p := RUN))"
+  apply (rule not_stuck_Seq)+
+    apply (rule not_stuck_If, simp_all add: Skip_def)
+  by (rule not_stuck_Basic)+
+
+lemma sched_await_post_inv: "\<lbrakk>(s\<^sub>c, s\<^sub>a) \<in> state_inv; s\<^sub>c' \<in> sched_await_post\<^sub>c s\<^sub>c k p; 
+      s\<^sub>a' \<in> sched_await_post\<^sub>a s\<^sub>a k p\<rbrakk> \<Longrightarrow> (s\<^sub>c', s\<^sub>a') \<in> schdule_post"
+  apply (simp add: state_inv_def, clarsimp)
+  by (case_tac "(cur\<^sub>c s\<^sub>c) (c2s conf k) = None", simp_all)
+
+lemma schedule_sim : "prog_sim_pre 
+      (Some 
+      (ATOMIC
+         IF (\<acute>cur\<^sub>c((c2s conf) k) \<noteq> None) THEN    
+           \<acute>partst\<^sub>c := \<acute>partst\<^sub>c(the (\<acute>cur\<^sub>c ((c2s conf) k)) := READY);;
+           \<acute>cur\<^sub>c := \<acute>cur\<^sub>c((c2s conf) k := None)
+         FI;;
+         \<acute>cur\<^sub>c := \<acute>cur\<^sub>c((c2s conf k) := Some p);;
+         \<acute>partst\<^sub>c := \<acute>partst\<^sub>c(p := RUN)
+       END))
+      (schedule\<^sub>c_rely k p) (schedule\<^sub>c_guar k p) 
+      state_inv (schedule_map k p) (schdule_pre k p) schdule_post
+      (Some 
+      (ATOMIC
+         IF (\<acute>cur\<^sub>a((c2s conf) k) \<noteq> None) THEN    
+           \<acute>partst\<^sub>a := \<acute>partst\<^sub>a(the (\<acute>cur\<^sub>a ((c2s conf) k)) := READY)
+          FI;;
+         \<acute>cur\<^sub>a := \<acute>cur\<^sub>a((c2s conf k) := Some p);;
+         \<acute>partst\<^sub>a := \<acute>partst\<^sub>a(p := RUN)
+       END))
+       schedule\<^sub>a_rely schedule\<^sub>a_guar"
+  apply (rule Await_Await_Sound, simp_all add: rel_eq_def Stable_def stable_alpha schedule_map_def)
+  using Stable_def stable_alpha apply fastforce
+  apply (simp add: related_transitions_def)
+  apply (metis (mono_tags, lifting) CollectD case_prodD state_inv_def)
+   apply (simp add: Skip_def not_stuck_Basic not_stuck_If not_stuck_Seq, clarsimp)
+  apply (rule_tac x = "sched_await_post\<^sub>c s\<^sub>c k p" in exI)
+  apply (rule conjI, rule schedc_await_sat_post, simp+)
+  apply (rule_tac x = "sched_await_post\<^sub>a s\<^sub>a k p" in exI)
+  apply (rule conjI, rule scheda_await_sat_post, simp+)
+  using sched_await_post_inv by force
+
+
+abbreviation "send\<^sub>c_rely k ch \<equiv> \<lbrace>\<ordfeminine>cur\<^sub>c (c2s conf k) = \<ordmasculine>cur\<^sub>c (c2s conf k) \<and>
+             (\<ordmasculine>qlock\<^sub>c ch = Some k \<longrightarrow> \<ordfeminine>qlock\<^sub>c ch = \<ordmasculine>qlock\<^sub>c ch \<and> \<ordfeminine>qbuf\<^sub>c ch = \<ordmasculine>qbuf\<^sub>c ch 
+            \<and> \<ordfeminine>qbufsize\<^sub>c ch = \<ordmasculine>qbufsize\<^sub>c ch \<and> \<ordfeminine>obsize\<^sub>c ch = \<ordmasculine>obsize\<^sub>c ch)\<rbrace> \<union> Id"
+
+abbreviation "send\<^sub>c_guar k ch \<equiv> 
+      {(s, s'). (qlock\<^sub>c s) ch = None \<and> s' = s \<lparr>qlock\<^sub>c := (qlock\<^sub>c s) (ch:= Some k)\<rparr>}
+    \<union> {(s, s'). \<exists>ms. (qlock\<^sub>c s) ch = Some k \<and> s' = s \<lparr>qbuf\<^sub>c := (qbuf\<^sub>c s) (ch := ms)\<rparr>}
+    \<union> {(s, s'). \<exists>n. (qlock\<^sub>c s) ch = Some k \<and> s' = s \<lparr>qbufsize\<^sub>c := (qbufsize\<^sub>c s) (ch :=  n)\<rparr>}
+    \<union> {(s, s'). \<exists>n. (qlock\<^sub>c s) ch = Some k \<and> s' = s \<lparr>qlock\<^sub>c := (qlock\<^sub>c s) (ch := None),
+                                                obsize\<^sub>c := (obsize\<^sub>c s) (ch := n) \<rparr>} \<union> Id"
+
+definition send_map :: "Core \<Rightarrow> Port \<Rightarrow> Message \<Rightarrow> State\<^sub>c com \<rightharpoonup> State\<^sub>a com"
+  where "send_map k p m = 
+        [ATOMIC
+          \<acute>qlock\<^sub>c := \<acute>qlock\<^sub>c (ch_srcqport conf p := None);;
+          \<acute>obsize\<^sub>c := \<acute>obsize\<^sub>c (ch_srcqport conf p := \<acute>qbufsize\<^sub>c (ch_srcqport conf p))
+         END
+      \<mapsto> ATOMIC
+          IF \<acute>qbufsize\<^sub>a (ch_srcqport conf p) < chmax conf (ch_srcqport conf p) THEN 
+            \<acute>qbuf\<^sub>a := \<acute>qbuf\<^sub>a (ch_srcqport conf p := \<acute>qbuf\<^sub>a (ch_srcqport conf p) @ [m]);;
+            \<acute>qbufsize\<^sub>a := \<acute>qbufsize\<^sub>a (ch_srcqport conf p := \<acute>qbufsize\<^sub>a (ch_srcqport conf p) + 1)
+          FI
+          END]"
+
+(*
+abbreviation "send_pre1 k p \<equiv> {(s\<^sub>c, s\<^sub>a). 
+  ((cur\<^sub>c s\<^sub>c) (c2s conf k) \<noteq> None \<and> port_of_part conf p (the ((cur\<^sub>c s\<^sub>c) (c2s conf k)))) \<and>
+  ((cur\<^sub>a s\<^sub>a) (c2s conf k) \<noteq> None \<and> port_of_part conf p (the ((cur\<^sub>a s\<^sub>a) (c2s conf k))))}"
+*)
+
+abbreviation "send_pre  \<equiv> state_inv"
+abbreviation "send_post \<equiv> state_inv"
+
+abbreviation "send\<^sub>a_rely \<equiv> UNIV"
+abbreviation "send\<^sub>a_guar \<equiv> UNIV"
+
+lemma senda_not_stuck: "not_stuck UNIV 
+      (IF \<acute>qbufsize\<^sub>a (ch_srcqport conf p) < chmax conf (ch_srcqport conf p) THEN 
+            \<acute>qbuf\<^sub>a := \<acute>qbuf\<^sub>a (ch_srcqport conf p := \<acute>qbuf\<^sub>a (ch_srcqport conf p) @ [m]);;
+            \<acute>qbufsize\<^sub>a := \<acute>qbufsize\<^sub>a (ch_srcqport conf p := \<acute>qbufsize\<^sub>a (ch_srcqport conf p) + 1)
+       FI)"
+  apply (rule not_stuck_If, simp_all add: Skip_def)
+   apply (rule not_stuck_Seq)
+  by (rule not_stuck_Basic)+
+
+
+abbreviation "sendc_unlock_await_post s ch  \<equiv> {s'. s' = s \<lparr>qlock\<^sub>c := (qlock\<^sub>c s) (ch := None),
+                                               obsize\<^sub>c := (obsize\<^sub>c s) (ch := (qbufsize\<^sub>c s ch)) \<rparr>}"
+
+abbreviation "sendc_unlock_await_mid s ch  \<equiv> {s'. s' = s \<lparr>qlock\<^sub>c := (qlock\<^sub>c s) (ch := None) \<rparr>}"
+
+lemma sendc_unlock_await_sat_post: "qlock\<^sub>c s\<^sub>c (ch_srcqport conf p) = Some k \<Longrightarrow>
+      \<turnstile> Await UNIV
+          (\<acute>qlock\<^sub>c := \<acute>qlock\<^sub>c(ch_srcqport conf p := None);;
+           \<acute>obsize\<^sub>c := \<acute>obsize\<^sub>c (ch_srcqport conf p :=\<acute>qbufsize\<^sub>c (ch_srcqport conf p)))
+      sat [{s\<^sub>c}, Id, send\<^sub>c_guar k (ch_srcqport conf p), sendc_unlock_await_post s\<^sub>c (ch_srcqport conf p)]"
+  apply (rule Await)        
+    apply (simp add: stable_def)+
+  apply (clarsimp, case_tac "V \<noteq> s\<^sub>c")
+   apply (rule Seq[where mid = "{}"])
+    apply (rule Basic)
+       apply (simp add: stable_def)+
+   apply (rule Basic)
+      apply (simp add: stable_def)+
+  apply (rule Seq[where mid = "sendc_unlock_await_mid s\<^sub>c  (ch_srcqport conf p)"])
+   apply (rule Basic)
+      apply (simp add: stable_def)+
+  apply (rule Basic, clarsimp)
+     apply blast
+  by (simp add: stable_def)+
+
+abbreviation "senda_await_post s m ch  \<equiv> {s'. 
+   (qbufsize\<^sub>a s ch < chmax conf ch \<longrightarrow> s' = s \<lparr> qbuf\<^sub>a := (qbuf\<^sub>a s) (ch := (qbuf\<^sub>a s ch) @ [m]),
+   qbufsize\<^sub>a := (qbufsize\<^sub>a s) (ch := (qbufsize\<^sub>a s ch) + 1)\<rparr>) \<and>
+   (qbufsize\<^sub>a s ch \<ge> chmax conf ch \<longrightarrow> s' = s)}"
+
+abbreviation "senda_await_mid s m ch  \<equiv> {s'. s' = s \<lparr> qbuf\<^sub>a := (qbuf\<^sub>a s) (ch := (qbuf\<^sub>a s ch) @ [m])\<rparr>}
+              \<inter> \<lbrace>(qbufsize\<^sub>a s) ch  < chmax conf ch\<rbrace>"
+
+lemma senda_await_sat_post: " 
+    \<turnstile> Await UNIV
+        (IF \<acute>qbufsize\<^sub>a (ch_srcqport conf p) < chmax conf (ch_srcqport conf p) THEN 
+          \<acute>qbuf\<^sub>a := \<acute>qbuf\<^sub>a(ch_srcqport conf p := \<acute>qbuf\<^sub>a (ch_srcqport conf p) @ [m]);; 
+          \<acute>qbufsize\<^sub>a := \<acute>qbufsize\<^sub>a(ch_srcqport conf p := Suc (\<acute>qbufsize\<^sub>a (ch_srcqport conf p))) FI) 
+      sat [{s\<^sub>a}, Id, send\<^sub>a_guar, senda_await_post s\<^sub>a m (ch_srcqport conf p)]"
+  apply (rule Await)
+    apply (simp add: stable_def)+
+  apply (clarsimp, case_tac "V \<noteq> s\<^sub>a")
+   apply (rule Cond)
+      apply (simp add: stable_def)+
+     apply (rule Seq[where mid = "{}"])
+      apply (rule Basic)
+         apply (simp add: stable_def)+
+     apply (rule Basic)
+        apply (simp add: stable_def)+
+    apply (simp add: Skip_def, rule Basic)
+       apply (simp add: stable_def)+
+  apply (rule Cond)
+     apply (simp add: stable_def)+
+    apply (rule Seq[where mid = "senda_await_mid s\<^sub>a m (ch_srcqport conf p)"])
+     apply (rule Basic, clarsimp)
+       apply (simp add: stable_def)+
+  apply (rule conjI, clarsimp)
+     apply (rule Basic, clarsimp)
+       apply (simp add: stable_def)+
+    apply (clarsimp, rule Basic)
+       apply (simp add: stable_def)+
+   apply (simp add: Skip_def, rule Basic, clarsimp)
+  by (simp add: stable_def)+
+
+abbreviation "send_unlock_pre k ch \<equiv> state_inv \<inter> 
+    {(s\<^sub>c, s\<^sub>a). qlock\<^sub>c s\<^sub>c ch = Some k \<and> 
+              (obsize\<^sub>c s\<^sub>c ch < chmax conf ch \<longrightarrow> qbufsize\<^sub>c s\<^sub>c ch = obsize\<^sub>c s\<^sub>c ch + 1) \<and> 
+              (obsize\<^sub>c s\<^sub>c ch \<ge> chmax conf ch \<longrightarrow> qbufsize\<^sub>c s\<^sub>c ch = obsize\<^sub>c s\<^sub>c ch)}"
+
+lemma send_await_post_inv: "\<lbrakk>(s\<^sub>c, s\<^sub>a) \<in> send_unlock_pre k ch; s\<^sub>c' \<in> sendc_unlock_await_post s\<^sub>c ch;
+      s\<^sub>a' \<in> senda_await_post s\<^sub>a m ch\<rbrakk> \<Longrightarrow> (s\<^sub>c', s\<^sub>a') \<in> send_post"
+  apply (case_tac "obsize\<^sub>c s\<^sub>c ch < chmax conf ch", simp add: state_inv_def, clarify)
+   apply presburger
+  apply (simp add: state_inv_def, clarify)
+  by presburger
+
+lemma send_unlock_sim: "prog_sim_pre (Some 
+      (ATOMIC
+          \<acute>qlock\<^sub>c := \<acute>qlock\<^sub>c (ch_srcqport conf p := None);;
+          \<acute>obsize\<^sub>c := \<acute>obsize\<^sub>c (ch_srcqport conf p := \<acute>qbufsize\<^sub>c (ch_srcqport conf p))
+       END))
+      (send\<^sub>c_rely k (ch_srcqport conf p)) (send\<^sub>c_guar k (ch_srcqport conf p)) 
+      state_inv (send_map k p m) (send_unlock_pre k (ch_srcqport conf p)) send_post
+      (Some 
+      (ATOMIC
+         IF \<acute>qbufsize\<^sub>a (ch_srcqport conf p) < chmax conf (ch_srcqport conf p) THEN 
+            \<acute>qbuf\<^sub>a := \<acute>qbuf\<^sub>a (ch_srcqport conf p := \<acute>qbuf\<^sub>a (ch_srcqport conf p) @ [m]);;
+            \<acute>qbufsize\<^sub>a := \<acute>qbufsize\<^sub>a (ch_srcqport conf p := \<acute>qbufsize\<^sub>a (ch_srcqport conf p) + 1)
+         FI
+       END))
+      send\<^sub>a_rely send\<^sub>a_guar"
+  apply (rule Await_Await_Sound)
+  using UNIV_I case_prodD colltrue_eq_univ rel_eq_def apply fastforce
+       apply (simp add: send_map_def)
+      apply (simp add: stable_alpha)
+     apply simp
+    apply (rule stable_conj, simp add: stable_alpha)
+    apply (simp add: Stable_def related_transitions_def)
+    apply auto[1]
+  using senda_not_stuck apply auto[1]
+  apply clarsimp
+  apply (rule_tac x = "sendc_unlock_await_post s\<^sub>c (ch_srcqport conf p)" in exI)
+  apply (rule conjI)
+  using sendc_unlock_await_sat_post apply auto[1]
+  apply (rule_tac x = "senda_await_post s\<^sub>a m (ch_srcqport conf p)" in exI)
+  apply (rule conjI)
+  using senda_await_sat_post apply auto[1]
+  by (clarsimp, rule send_await_post_inv, simp_all)
+
+abbreviation "send_sim_mid1 k ch \<equiv> send_unlock_pre k ch"
+abbreviation "send_sim_mid2 k ch \<equiv> state_inv \<inter> {(s\<^sub>c, s\<^sub>a). qlock\<^sub>c s\<^sub>c ch = Some k \<and> qbufsize\<^sub>c s\<^sub>c ch = obsize\<^sub>c s\<^sub>c ch}"
+
+
+lemma send_sim_none1: "prog_sim_pre (Some 
+      (AWAIT \<acute>qlock\<^sub>c (ch_srcqport conf p) = None THEN
+        \<acute>qlock\<^sub>c := \<acute>qlock\<^sub>c (ch_srcqport conf p := Some k)
+       END))
+      (send\<^sub>c_rely k (ch_srcqport conf p)) (send\<^sub>c_guar k (ch_srcqport conf p)) 
+      state_inv Map.empty send_pre (send_sim_mid2 k (ch_srcqport conf p))
+      None
+      send\<^sub>a_rely send\<^sub>a_guar"
+  apply (rule Await_None_Sound)
+       apply simp+
+     apply (simp add: Stable_def related_transitions_def)+
+    apply auto[1]
+   apply simp
+  apply clarsimp
+  apply (rule Await)
+    apply (simp add: stable_def)+
+  apply (clarsimp, rule Basic, clarsimp)
+     apply (simp add: state_inv_def)
+     apply auto[1]
+    apply (simp add: stable_def)+
+   apply auto[1]
+  by (simp add: stable_def)
+
+abbreviation "send_sim_none_if_mid k ch \<equiv> state_inv \<inter> {(s\<^sub>c, s\<^sub>a). qbufsize\<^sub>c s\<^sub>c ch < chmax conf ch}
+             \<inter> {(s\<^sub>c, s\<^sub>a). qlock\<^sub>c s\<^sub>c ch = Some k \<and> qbufsize\<^sub>c s\<^sub>c ch = obsize\<^sub>c s\<^sub>c ch}"
+
+lemma send_sim_none2: "prog_sim_pre (Some 
+      (IF \<acute>qbufsize\<^sub>c (ch_srcqport conf p) < chmax conf (ch_srcqport conf p) THEN 
+         \<acute>qbuf\<^sub>c := \<acute>qbuf\<^sub>c (ch_srcqport conf p := \<acute>qbuf\<^sub>c (ch_srcqport conf p) @ [m]);;
+         \<acute>qbufsize\<^sub>c := \<acute>qbufsize\<^sub>c (ch_srcqport conf p := \<acute>qbufsize\<^sub>c (ch_srcqport conf p) + 1)
+       FI))
+      (send\<^sub>c_rely k (ch_srcqport conf p)) (send\<^sub>c_guar k (ch_srcqport conf p))
+      state_inv Map.empty (send_sim_mid2 k (ch_srcqport conf p)) (send_sim_mid1 k (ch_srcqport conf p))
+      None
+      send\<^sub>a_rely send\<^sub>a_guar"
+  apply auto
+  apply (rule If_Comm_Branch_Sound)
+        apply simp+
+      apply (simp add: Stable_def related_transitions_def)
+       apply auto
+   apply (rule_tac \<zeta>\<^sub>1 = Map.empty and \<gamma>\<^sub>1 = "send_sim_none_if_mid k (ch_srcqport conf p)" in Seq_Skip_Sound)
+      apply blast
+     apply simp
+    apply (rule Basic_None_Sound)
+         apply blast+
+       apply (simp add: Stable_def related_transitions_def)
+       apply fastforce
+      apply (simp add: Stable_def related_transitions_def)
+      apply fastforce
+     apply (simp add: state_inv_def)
+     apply auto[1]
+    apply simp
+   apply (rule Basic_None_Sound)
+        apply blast+
+      apply (simp add: Stable_def related_transitions_def)
+      apply fastforce
+     apply (simp add: Stable_def related_transitions_def)
+     apply fastforce
+    apply (simp add: state_inv_def)
+    apply auto[1]
+   apply simp
+  apply (simp add: Skip_def, rule Basic_None_Sound)
+       apply blast+
+     apply (simp add: Stable_def related_transitions_def)
+     apply fastforce
+    apply (simp add: Stable_def related_transitions_def)
+    apply fastforce
+   apply (simp add: state_inv_def)
+  by auto
+
+lemma send_sim: "prog_sim_pre (Some 
+      (AWAIT \<acute>qlock\<^sub>c (ch_srcqport conf p) = None THEN
+        \<acute>qlock\<^sub>c := \<acute>qlock\<^sub>c (ch_srcqport conf p := Some k)
+       END;;
+       IF \<acute>qbufsize\<^sub>c (ch_srcqport conf p) < chmax conf (ch_srcqport conf p) THEN 
+         \<acute>qbuf\<^sub>c := \<acute>qbuf\<^sub>c (ch_srcqport conf p := \<acute>qbuf\<^sub>c (ch_srcqport conf p) @ [m]);;
+         \<acute>qbufsize\<^sub>c := \<acute>qbufsize\<^sub>c (ch_srcqport conf p := \<acute>qbufsize\<^sub>c (ch_srcqport conf p) + 1)
+       FI;;
+       ATOMIC
+         \<acute>qlock\<^sub>c := \<acute>qlock\<^sub>c (ch_srcqport conf p := None);;
+         \<acute>obsize\<^sub>c := \<acute>obsize\<^sub>c (ch_srcqport conf p := \<acute>qbufsize\<^sub>c (ch_srcqport conf p))
+       END))
+      (send\<^sub>c_rely k (ch_srcqport conf p)) (send\<^sub>c_guar k (ch_srcqport conf p)) 
+      state_inv (send_map k p m) send_pre send_post
+      (Some 
+      (ATOMIC
+         IF \<acute>qbufsize\<^sub>a (ch_srcqport conf p) < chmax conf (ch_srcqport conf p) THEN 
+            \<acute>qbuf\<^sub>a := \<acute>qbuf\<^sub>a (ch_srcqport conf p := \<acute>qbuf\<^sub>a (ch_srcqport conf p) @ [m]);;
+            \<acute>qbufsize\<^sub>a := \<acute>qbufsize\<^sub>a (ch_srcqport conf p := \<acute>qbufsize\<^sub>a (ch_srcqport conf p) + 1)
+         FI
+       END))
+      send\<^sub>a_rely send\<^sub>a_guar"
+  apply (rule_tac \<zeta>\<^sub>1 = Map.empty and \<gamma>\<^sub>1 = "send_sim_mid1 k (ch_srcqport conf p)" in Seq_Skip_Sound)
+    apply (simp add: send_map_def)+
+   apply (rule_tac \<zeta>\<^sub>1 = Map.empty and \<gamma>\<^sub>1 = "send_sim_mid2 k (ch_srcqport conf p)" in Seq_Skip_Sound)
+      apply simp+
+  using send_sim_none1 apply auto[1]
+  using send_sim_none2 apply auto[1]
+  using send_unlock_sim by auto
+
+
+abbreviation "recv\<^sub>c_rely k ch \<equiv> \<lbrace>\<ordfeminine>cur\<^sub>c (c2s conf k) = \<ordmasculine>cur\<^sub>c (c2s conf k) \<and>
+             (\<ordmasculine>qlock\<^sub>c ch = Some k \<longrightarrow> \<ordfeminine>qlock\<^sub>c ch = \<ordmasculine>qlock\<^sub>c ch \<and> \<ordfeminine>qbuf\<^sub>c ch = \<ordmasculine>qbuf\<^sub>c ch 
+            \<and> \<ordfeminine>qbufsize\<^sub>c ch = \<ordmasculine>qbufsize\<^sub>c ch \<and> \<ordfeminine>obsize\<^sub>c ch = \<ordmasculine>obsize\<^sub>c ch)\<rbrace> \<union> Id"
+
+abbreviation "recv\<^sub>c_guar k ch \<equiv> 
+      {(s, s'). (qlock\<^sub>c s) ch = None \<and> s' = s \<lparr>qlock\<^sub>c := (qlock\<^sub>c s) (ch:= Some k)\<rparr>}
+    \<union> {(s, s'). \<exists>ms. (qlock\<^sub>c s) ch = Some k \<and> s' = s \<lparr>qbuf\<^sub>c := (qbuf\<^sub>c s) (ch := ms)\<rparr>}
+    \<union> {(s, s'). \<exists>n. (qlock\<^sub>c s) ch = Some k \<and> s' = s \<lparr>qbufsize\<^sub>c := (qbufsize\<^sub>c s) (ch :=  n)\<rparr>}
+    \<union> {(s, s'). \<exists>n. (qlock\<^sub>c s) ch = Some k \<and> s' = s \<lparr>qlock\<^sub>c := (qlock\<^sub>c s) (ch := None),
+                                                obsize\<^sub>c := (obsize\<^sub>c s) (ch := n) \<rparr>} \<union> Id"
+
+definition recv_map :: "Core \<Rightarrow> Port  \<Rightarrow> State\<^sub>c com \<rightharpoonup> State\<^sub>a com"
+  where "recv_map k p = 
+        [ATOMIC
+          \<acute>qlock\<^sub>c := \<acute>qlock\<^sub>c (ch_destqport conf p := None);;
+          \<acute>obsize\<^sub>c := \<acute>obsize\<^sub>c (ch_destqport conf p := \<acute>qbufsize\<^sub>c (ch_destqport conf p))
+         END
+      \<mapsto> ATOMIC
+           IF \<acute>qbufsize\<^sub>a (ch_destqport conf p) > 0 THEN 
+             \<acute>qbuf\<^sub>a := \<acute>qbuf\<^sub>a (ch_destqport conf p := tl (\<acute>qbuf\<^sub>a (ch_destqport conf p)));;
+             \<acute>qbufsize\<^sub>a := \<acute>qbufsize\<^sub>a (ch_destqport conf p := \<acute>qbufsize\<^sub>a (ch_destqport conf p) - 1)
+           FI
+         END]"
+
+(*
+abbreviation "send_pre1 k p \<equiv> {(s\<^sub>c, s\<^sub>a). 
+  ((cur\<^sub>c s\<^sub>c) (c2s conf k) \<noteq> None \<and> port_of_part conf p (the ((cur\<^sub>c s\<^sub>c) (c2s conf k)))) \<and>
+  ((cur\<^sub>a s\<^sub>a) (c2s conf k) \<noteq> None \<and> port_of_part conf p (the ((cur\<^sub>a s\<^sub>a) (c2s conf k))))}"
+*)
+
+abbreviation "recv_pre  \<equiv> state_inv"
+abbreviation "recv_post \<equiv> state_inv"
+
+abbreviation "recv\<^sub>a_rely \<equiv> UNIV"
+abbreviation "recv\<^sub>a_guar \<equiv> UNIV"
+
+lemma recva_not_stuck: "not_stuck UNIV 
+      (IF \<acute>qbufsize\<^sub>a (ch_destqport conf p) > 0 THEN 
+             \<acute>qbuf\<^sub>a := \<acute>qbuf\<^sub>a (ch_destqport conf p := tl (\<acute>qbuf\<^sub>a (ch_destqport conf p)));;
+             \<acute>qbufsize\<^sub>a := \<acute>qbufsize\<^sub>a (ch_destqport conf p := \<acute>qbufsize\<^sub>a (ch_destqport conf p) - 1)
+       FI)"
+  apply (rule not_stuck_If, simp_all add: Skip_def)
+   apply (rule not_stuck_Seq)
+  by (rule not_stuck_Basic)+
+
+abbreviation "recvc_unlock_await_post s ch  \<equiv> {s'. s' = s \<lparr>qlock\<^sub>c := (qlock\<^sub>c s) (ch := None),
+                                               obsize\<^sub>c := (obsize\<^sub>c s) (ch := (qbufsize\<^sub>c s ch)) \<rparr>}"
+
+abbreviation "recvc_unlock_await_mid s ch  \<equiv> {s'. s' = s \<lparr>qlock\<^sub>c := (qlock\<^sub>c s) (ch := None) \<rparr>}"
+
+lemma recvc_unlock_await_sat_post: "qlock\<^sub>c s\<^sub>c (ch_destqport conf p) = Some k \<Longrightarrow>
+      \<turnstile> Await UNIV
+          (\<acute>qlock\<^sub>c := \<acute>qlock\<^sub>c(ch_destqport conf p := None);;
+           \<acute>obsize\<^sub>c := \<acute>obsize\<^sub>c (ch_destqport conf p :=\<acute>qbufsize\<^sub>c (ch_destqport conf p)))
+      sat [{s\<^sub>c}, Id, recv\<^sub>c_guar k (ch_destqport conf p), recvc_unlock_await_post s\<^sub>c (ch_destqport conf p)]"
+  apply (rule Await)        
+    apply (simp add: stable_def)+
+  apply (clarsimp, case_tac "V \<noteq> s\<^sub>c")
+   apply (rule Seq[where mid = "{}"])
+    apply (rule Basic)
+       apply (simp add: stable_def)+
+   apply (rule Basic)
+      apply (simp add: stable_def)+
+  apply (rule Seq[where mid = "recvc_unlock_await_mid s\<^sub>c (ch_destqport conf p)"])
+   apply (rule Basic)
+      apply (simp add: stable_def)+
+  apply (rule Basic, clarsimp)
+     apply blast
+  by (simp add: stable_def)+
+
+abbreviation "recva_await_post s ch  \<equiv> {s'. 
+   (qbufsize\<^sub>a s ch > 0 \<longrightarrow> s' = s \<lparr> qbuf\<^sub>a := (qbuf\<^sub>a s) (ch := tl (qbuf\<^sub>a s ch)),
+    qbufsize\<^sub>a := (qbufsize\<^sub>a s) (ch := (qbufsize\<^sub>a s ch) - 1)\<rparr>) \<and>
+   (qbufsize\<^sub>a s ch = 0 \<longrightarrow> s' = s)}"
+
+abbreviation "recva_await_mid s ch  \<equiv> {s'. s' = s \<lparr> qbuf\<^sub>a := (qbuf\<^sub>a s) (ch := tl (qbuf\<^sub>a s ch))\<rparr>}
+              \<inter> \<lbrace>(qbufsize\<^sub>a s) ch > 0\<rbrace>"
+
+lemma recva_await_sat_post: " 
+    \<turnstile> Await UNIV
+        (IF \<acute>qbufsize\<^sub>a (ch_destqport conf p) > 0 THEN 
+          \<acute>qbuf\<^sub>a := \<acute>qbuf\<^sub>a (ch_destqport conf p := tl (\<acute>qbuf\<^sub>a (ch_destqport conf p)));;
+          \<acute>qbufsize\<^sub>a := \<acute>qbufsize\<^sub>a (ch_destqport conf p := \<acute>qbufsize\<^sub>a (ch_destqport conf p) - 1)
+         FI) 
+      sat [{s\<^sub>a}, Id, recv\<^sub>a_guar, recva_await_post s\<^sub>a  (ch_destqport conf p)]"
+  apply (rule Await)
+    apply (simp add: stable_def)+
+  apply (clarsimp, case_tac "V \<noteq> s\<^sub>a")
+   apply (rule Cond)
+      apply (simp add: stable_def)+
+     apply (rule Seq[where mid = "{}"])
+      apply (rule Basic)
+         apply (simp add: stable_def)+
+     apply (rule Basic)
+        apply (simp add: stable_def)+
+    apply (simp add: Skip_def, rule Basic)
+       apply (simp add: stable_def)+
+  apply (rule Cond)
+     apply (simp add: stable_def)+
+    apply (rule Seq[where mid = "recva_await_mid s\<^sub>a (ch_destqport conf p)"])
+     apply (rule Basic, clarsimp)
+       apply (simp add: stable_def)+
+  apply (rule conjI, clarsimp)
+     apply (rule Basic, clarsimp)
+       apply (simp add: stable_def)+
+    apply (clarsimp, rule Basic)
+       apply (simp add: stable_def)+
+   apply (simp add: Skip_def, rule Basic, clarsimp)
+  by (simp add: stable_def)+
+
+abbreviation "recv_unlock_pre k ch \<equiv> state_inv \<inter> 
+    {(s\<^sub>c, s\<^sub>a). qlock\<^sub>c s\<^sub>c ch = Some k \<and> 
+              (obsize\<^sub>c s\<^sub>c ch > 0  \<longrightarrow> qbufsize\<^sub>c s\<^sub>c ch = obsize\<^sub>c s\<^sub>c ch - 1) \<and> 
+              (obsize\<^sub>c s\<^sub>c ch = 0  \<longrightarrow> qbufsize\<^sub>c s\<^sub>c ch = obsize\<^sub>c s\<^sub>c ch)}"
+
+lemma recv_await_post_inv: "\<lbrakk>(s\<^sub>c, s\<^sub>a) \<in> recv_unlock_pre k ch; s\<^sub>c' \<in> recvc_unlock_await_post s\<^sub>c ch;
+      s\<^sub>a' \<in> recva_await_post s\<^sub>a ch\<rbrakk> \<Longrightarrow> (s\<^sub>c', s\<^sub>a') \<in> recv_post"
+  apply (case_tac "obsize\<^sub>c s\<^sub>c ch > 0", simp add: state_inv_def, clarify)
+   apply presburger
+  apply (simp add: state_inv_def, clarify)
   by force
 
-lemma Schedule_sat_SCE: "sc_p_sat (the (body_e (Schedule k p))) (Schedule k p)"
-  apply (simp add: body_def Schedule_def)
-  apply (rule sc_p_sat.Seq)
-   apply (rule sc_p_sat.Cond)
-    apply (rule_tac pre = "\<lbrace>p2s conf p = c2s conf k \<and> p2s conf (the (\<acute>cur (c2s conf k))) = c2s conf k\<rbrace>" 
-          and rely = Id and post = "\<lbrace>True\<rbrace>" and guar = "\<lbrace>\<ordfeminine>qbuf = \<ordmasculine>qbuf \<and> \<ordfeminine>qbufsize = \<ordmasculine>qbufsize \<and> 
-          \<ordfeminine>cur = \<ordmasculine>cur(c2s conf k := None) \<and> \<ordfeminine>partst = \<ordmasculine>partst(the (\<ordmasculine>cur (c2s conf k)) := READY) \<and> 
-          (\<forall>p. p2s conf p \<noteq> c2s conf k \<longrightarrow> \<ordfeminine>partst  p = \<ordmasculine>partst p )\<rbrace>" in sc_p_sat.Await)
-      apply (rule rghoare_p.Await, clarsimp)
-        apply (simp add: stable_def)+
-      apply (rule allI)
-  using Schedule_sat_SCE_h1 apply auto[1]
+lemma recv_unlock_sim: "prog_sim_pre (Some 
+      (ATOMIC
+          \<acute>qlock\<^sub>c := \<acute>qlock\<^sub>c (ch_destqport conf p := None);;
+          \<acute>obsize\<^sub>c := \<acute>obsize\<^sub>c (ch_destqport conf p := \<acute>qbufsize\<^sub>c (ch_destqport conf p))
+       END))
+      (recv\<^sub>c_rely k (ch_destqport conf p)) (recv\<^sub>c_guar k (ch_destqport conf p)) 
+      state_inv (recv_map k p) (recv_unlock_pre k (ch_destqport conf p)) send_post
+      (Some 
+      (ATOMIC
+         IF \<acute>qbufsize\<^sub>a (ch_destqport conf p) > 0 THEN 
+             \<acute>qbuf\<^sub>a := \<acute>qbuf\<^sub>a (ch_destqport conf p := tl (\<acute>qbuf\<^sub>a (ch_destqport conf p)));;
+             \<acute>qbufsize\<^sub>a := \<acute>qbufsize\<^sub>a (ch_destqport conf p := \<acute>qbufsize\<^sub>a (ch_destqport conf p) - 1)
+         FI
+       END))
+      send\<^sub>a_rely send\<^sub>a_guar"
+  apply (rule Await_Await_Sound)
+  using UNIV_I case_prodD colltrue_eq_univ rel_eq_def apply fastforce
+       apply (simp add: recv_map_def)
+      apply (simp add: stable_alpha)
      apply simp
-    apply (simp add: domevt_def get_evt_core_def Schedule_def label_def get_evt_el_def get_evt_label_def, clarify)
-     apply (case_tac u)
-      apply (case_tac "p2s conf x1 = c2s conf k")
-       apply (simp add: interf_def state_equiv_def state_obs_sched_def state_obs_part_def s0_init System_Init_def)
-        apply (smt (verit, best) State.ext_inject State.update_convs(1) State.update_convs(3) State.update_convs(4) 
-              fst_conv fun_upd_other fun_upd_same obs_cap_equiv1)
-      apply (metis obs_cap_equiv1 state_equiv_def state_obs.simps(1) state_obs_part_def)
-     apply (simp add: System_Init_def s0_init state_equiv_def state_obs_sched_def)
-  using state_equiv_def state_obs.simps(3) apply presburger
-   apply (rule sc_p_sat.Basic, simp)
-    apply (rule_tac pre = "\<lbrace>p2s conf p = c2s conf k \<and> \<acute>cur (c2s conf k) = None\<rbrace>" 
-          and rely = Id and post = "\<lbrace>True\<rbrace>" and guar = "\<lbrace>\<ordfeminine>qbuf = \<ordmasculine>qbuf \<and> \<ordfeminine>qbufsize = \<ordmasculine>qbufsize \<and>  
-          \<ordfeminine>cur = \<ordmasculine>cur(c2s conf k := Some p) \<and> \<ordfeminine>partst = \<ordmasculine>partst(the (\<ordfeminine>cur(c2s conf k)) := RUN) \<and> 
-          (\<forall>p. p2s conf p \<noteq> c2s conf k \<longrightarrow> \<ordfeminine>partst  p = \<ordmasculine>partst p)\<rbrace>" in sc_p_sat.Await)
-    apply (rule rghoare_p.Await, simp)
-      apply (simp add: stable_def)+
-    apply (rule allI)
-  using Schedule_sat_SCE_h2 apply auto[1]
-    apply simp
-   apply (simp add: domevt_def get_evt_core_def Schedule_def label_def get_evt_el_def get_evt_label_def, clarify)
-   apply (case_tac u)
-     apply (case_tac "p2s conf x1 = c2s conf k")
-      apply (simp add: interf_def state_equiv_def state_obs_sched_def state_obs_part_def s0_init System_Init_def)
-      apply (smt (verit, best) State.ext_inject State.update_convs(1) State.update_convs(3) State.update_convs(4) 
-              fst_conv fun_upd_other fun_upd_same obs_cap_equiv1)
-     apply (metis obs_cap_equiv1 state_equiv_def state_obs.simps(1) state_obs_part_def)
-    apply (simp add: System_Init_def s0_init state_equiv_def state_obs_sched_def)
-  using state_equiv_def state_obs.simps(3) by presburger
+    apply (rule stable_conj, simp add: stable_alpha)
+    apply (simp add: Stable_def related_transitions_def)
+    apply auto[1]
+  using recva_not_stuck apply auto[1]
+  apply clarsimp
+  apply (rule_tac x = "recvc_unlock_await_post s\<^sub>c (ch_destqport conf p)" in exI)
+  apply (rule conjI)
+  using recvc_unlock_await_sat_post apply auto[1]
+  apply (rule_tac x = "recva_await_post s\<^sub>a (ch_destqport conf p)" in exI)
+  apply (rule conjI)
+  using recva_await_sat_post apply auto[1]
+  by (clarsimp, rule recv_await_post_inv, simp_all)
 
-lemma Send_Que_sat_SCE_h1: "\<turnstile>\<^sub>I Some (\<lbrace>True \<rbrace> \<acute>qbuf := \<acute>qbuf(ch_srcqport conf p := \<acute>qbuf (ch_srcqport conf p) @ [m]) ;;
-                              \<lbrace>True \<rbrace> \<acute>qbufsize := \<acute>qbufsize (ch_srcqport conf p := Suc (\<acute>qbufsize (ch_srcqport conf p))))
-     sat\<^sub>p [\<lbrace>is_src_qport conf p \<and> (\<exists>y. \<acute>cur (c2s conf k) = Some y) \<and> port_of_part conf p (the (\<acute>cur (c2s conf k)))\<rbrace> 
-            \<inter> {V} \<inter> \<lbrace>\<acute>qbufsize (ch_srcqport conf p) < chmax conf (ch_srcqport conf p)\<rbrace>, 
-            {(s, t). s = t}, UNIV, \<lbrace>\<acute>cur = cur V \<and> \<acute>partst = partst V \<and> (is_src_qport conf p \<and> 
-            (\<exists>y. cur V (c2s conf k) = Some y) \<and> port_of_part conf p (the (cur V (c2s conf k))) \<longrightarrow>
-            (\<forall>c. c \<noteq> ch_srcqport conf p \<longrightarrow> \<acute>qbuf c = qbuf V c \<and> \<acute>qbufsize c = qbufsize V c) \<and>
-            (qbufsize V (ch_srcqport conf p) < chmax conf (ch_srcqport conf p) \<longrightarrow> 
-            \<acute>qbufsize (ch_srcqport conf p) = Suc (qbufsize V (ch_srcqport conf p))) \<and>
-            (chmax conf (ch_srcqport conf p) \<le> qbufsize V (ch_srcqport conf p) \<longrightarrow> 
-            \<acute>qbuf = qbuf V \<and> \<acute>qbufsize = qbufsize V)) \<and> ((is_src_qport conf p \<longrightarrow> cur V (c2s conf k) = None 
-            \<or> \<not> port_of_part conf p (the (cur V (c2s conf k)))) \<longrightarrow> \<acute>qbuf = qbuf V \<and> \<acute>qbufsize = qbufsize V)\<rbrace>]"
-  apply(case_tac "is_src_qport conf p \<and> (\<exists>y. (cur V) ((c2s conf) k) = Some y) \<and> port_of_part conf p 
-      (the ((cur V) ((c2s conf) k)))\<and> (qbufsize V) (ch_srcqport conf p) < chmax conf (ch_srcqport conf p)")
+abbreviation "recv_sim_mid1 k ch \<equiv> recv_unlock_pre k ch"
+abbreviation "recv_sim_mid2 k ch \<equiv> state_inv \<inter> {(s\<^sub>c, s\<^sub>a). qlock\<^sub>c s\<^sub>c ch = Some k \<and> qbufsize\<^sub>c s\<^sub>c ch = obsize\<^sub>c s\<^sub>c ch}"
+
+
+lemma recv_sim_none1: "prog_sim_pre (Some 
+      (AWAIT \<acute>qlock\<^sub>c (ch_destqport conf p) = None THEN
+        \<acute>qlock\<^sub>c := \<acute>qlock\<^sub>c (ch_destqport conf p := Some k)
+       END))
+      (recv\<^sub>c_rely k (ch_destqport conf p)) (recv\<^sub>c_guar k (ch_destqport conf p)) 
+      state_inv Map.empty recv_pre (recv_sim_mid2 k (ch_destqport conf p))
+      None
+      recv\<^sub>a_rely recv\<^sub>a_guar"
+  apply (rule Await_None_Sound)
+       apply simp+
+     apply (simp add: Stable_def related_transitions_def)+
+    apply auto[1]
    apply simp
-   apply(rule rghoare_p.Seq[where mid="{s. s = V\<lparr>qbuf := (qbuf V)(ch_srcqport conf p := (qbuf V) (ch_srcqport conf p) @ [m])\<rparr>}"])
-    apply(rule rghoare_p.Basic)
-        apply auto[1]
-       apply(simp add: stable_def)+
-   apply(rule rghoare_p.Basic, simp)
-      apply auto[1]
-     apply(simp add: stable_def)+
-  apply(rule rghoare_p.Seq[where mid="{}"])
-   apply(rule rghoare_p.Basic, simp)
-      apply(simp add:stable_def)+
-      apply fastforce
-     apply simp
+  apply clarsimp
+  apply (rule Await)
     apply (simp add: stable_def)+
-  apply(rule rghoare_p.Basic)
-      apply(simp add:stable_def)+
-  done
+  apply (clarsimp, rule Basic, clarsimp)
+     apply (simp add: state_inv_def)
+     apply auto[1]
+    apply (simp add: stable_def)+
+   apply auto[1]
+  by (simp add: stable_def)
 
-lemma Send_Que_sat_SCE: "sc_p_sat (the (body_e (Send_Que_Message k p m))) (Send_Que_Message k p m)"
-  apply (simp add: body_def Send_Que_Message_def)
-  apply (rule_tac pre = "\<lbrace>is_src_qport conf p \<and> (\<exists>y. \<acute>cur (c2s conf k) = Some y) \<and> port_of_part conf p (the (\<acute>cur (c2s conf k)))\<rbrace>" 
-          and rely = Id and post = "\<lbrace>True\<rbrace>" and guar = "\<lbrace>\<ordfeminine>cur = \<ordmasculine>cur \<and> \<ordfeminine>partst = \<ordmasculine>partst \<and> 
-          ((is_src_qport conf p \<and> \<ordmasculine>cur ((c2s conf) k) \<noteq> None \<and> port_of_part conf p (the (\<ordmasculine>cur ((c2s conf) k)))) 
-          \<longrightarrow> (\<forall>c. c \<noteq> ch_srcqport conf p \<longrightarrow> \<ordfeminine>qbuf c = \<ordmasculine>qbuf c \<and> \<ordfeminine>qbufsize c = \<ordmasculine>qbufsize c) \<and> 
-          (\<ordmasculine>qbufsize (ch_srcqport conf p) < chmax conf (ch_srcqport conf p) \<longrightarrow> 
-          \<ordfeminine>qbufsize (ch_srcqport conf p) = \<ordmasculine>qbufsize (ch_srcqport conf p) + 1) \<and>
-          (\<ordmasculine>qbufsize (ch_srcqport conf p) \<ge> chmax conf (ch_srcqport conf p) \<longrightarrow> 
-          \<ordfeminine>qbuf = \<ordmasculine>qbuf \<and> \<ordfeminine>qbufsize  = \<ordmasculine>qbufsize)) \<and> ((\<not>(is_src_qport conf p \<and> 
-          \<ordmasculine>cur ((c2s conf) k) \<noteq> None \<and> port_of_part conf p (the (\<ordmasculine>cur ((c2s conf) k)))))\<longrightarrow> 
-          (\<ordfeminine>qbuf  = \<ordmasculine>qbuf  \<and> \<ordfeminine>qbufsize  = \<ordmasculine>qbufsize))\<rbrace>" in sc_p_sat.Await)
-    apply (rule rghoare_p.Await, simp)
-      apply (simp add: stable_def)+
-    apply (rule allI)
-    apply (rule rghoare_p.Cond, simp, simp add: stable_def)
-  using Send_Que_sat_SCE_h1 apply auto[1]
-     apply (rule rghoare_p.Basic)
-         apply blast
-        apply auto[1]
-       apply simp
-      apply (simp add: stable_def)+
-  apply (simp add: domevt_def get_evt_core_def Send_Que_Message_def label_def get_evt_el_def get_evt_label_def, clarify)
-  apply (case_tac u)
-    apply (simp add: state_equiv_def state_obs_part_def)
-    apply (rule s0_update_help)
-     apply (smt (z3) State.ext_inject State.surjective State.update_convs(3) State.update_convs(4))
-    apply (rule obs_cap_equiv, clarsimp)
-    apply (subgoal_tac "qbufsize s1 c = qbufsize s2 c")
-     apply (case_tac "c = ch_srcqport conf p")
-      apply (erule impE)
-       apply (metis ch_chonn_help2 interf_def noninterf_def)
-      apply (case_tac "qbufsize s1 c < chmax conf (ch_srcqport conf p)", simp)
-      apply (case_tac "qbufsize s2 c < chmax conf (ch_srcqport conf p)")
-       apply linarith
-      apply (metis linorder_not_le)
-     apply presburger
-    apply (metis (no_types, lifting) State.ext_inject State.surjective State.update_convs(3) obs_cap_part_def)
-   apply (simp add: state_equiv_def state_obs_sched_def)
-  using state_equiv_def state_obs.simps(3) by presburger
+abbreviation "recv_sim_none_if_mid k ch \<equiv> state_inv \<inter> {(s\<^sub>c, s\<^sub>a). qbufsize\<^sub>c s\<^sub>c ch > 0}
+             \<inter> {(s\<^sub>c, s\<^sub>a). qlock\<^sub>c s\<^sub>c ch = Some k \<and> qbufsize\<^sub>c s\<^sub>c ch = obsize\<^sub>c s\<^sub>c ch}"
 
-lemma Recv_Que_sat_SCE_h1: "\<turnstile>\<^sub>I Some (\<lbrace>True\<rbrace> \<acute>qbuf := \<acute>qbuf(ch_destqport conf p := tl (\<acute>qbuf (ch_destqport conf p)));;
-                         \<lbrace>True \<rbrace>\<acute>qbufsize := \<acute>qbufsize (ch_destqport conf p := \<acute>qbufsize (ch_destqport conf p) - Suc 0))
-  sat\<^sub>p [\<lbrace>is_dest_qport conf p \<and> (\<exists>y. \<acute>cur (c2s conf k) = Some y) \<and> port_of_part conf p (the (\<acute>cur (c2s conf k)))\<rbrace> 
-        \<inter> \<lbrace>0 < \<acute>qbufsize (ch_destqport conf p)\<rbrace> \<inter> {V}, {(s, t). s = t}, UNIV, \<lbrace>\<acute>cur = cur V \<and>
-       \<acute>partst = partst V \<and> (is_dest_qport conf p \<and> (\<exists>y. cur V (c2s conf k) = Some y) \<and> 
-        port_of_part conf p (the (cur V (c2s conf k))) \<longrightarrow> (\<forall>c. c \<noteq> ch_destqport conf p \<longrightarrow> 
-        \<acute>qbuf c = qbuf V c \<and> \<acute>qbufsize c = qbufsize V c) \<and> (0 < qbufsize V (ch_destqport conf p) \<longrightarrow> 
-        \<acute>qbufsize (ch_destqport conf p) = qbufsize V (ch_destqport conf p) - Suc 0) \<and> 
-         (qbufsize V (ch_destqport conf p) = 0 \<longrightarrow> \<acute>qbuf = qbuf V \<and> \<acute>qbufsize = qbufsize V)) \<and>
-         ((is_dest_qport conf p \<longrightarrow> cur V (c2s conf k) = None \<or> \<not> port_of_part conf p (the (cur V (c2s conf k)))) 
-          \<longrightarrow> \<acute>qbuf = qbuf V \<and> \<acute>qbufsize = qbufsize V)\<rbrace>]"
-  apply(case_tac "is_dest_qport conf p \<and> (\<exists>y. (cur V) ((c2s conf) k) = Some y) \<and> 
-        port_of_part conf p (the ((cur V) ((c2s conf) k))) \<and> 0 < (qbufsize V) (ch_destqport conf p)")
-   apply simp
-   apply(rule rghoare_p.Seq[where mid="{s. s = V\<lparr>qbuf := (qbuf V)(ch_destqport conf p := tl ((qbuf V) (ch_destqport conf p)))\<rparr>}"])
-    apply(rule rghoare_p.Basic)
-        apply auto[1]
-       apply auto[1]
+lemma recv_sim_none2: "prog_sim_pre (Some 
+      (IF \<acute>qbufsize\<^sub>c (ch_destqport conf p) > 0 THEN 
+        \<acute>qbuf\<^sub>c := \<acute>qbuf\<^sub>c (ch_destqport conf p := tl (\<acute>qbuf\<^sub>c (ch_destqport conf p)));;
+        \<acute>qbufsize\<^sub>c := \<acute>qbufsize\<^sub>c (ch_destqport conf p := \<acute>qbufsize\<^sub>c (ch_destqport conf p) - 1)
+      FI))
+      (recv\<^sub>c_rely k (ch_destqport conf p)) (recv\<^sub>c_guar k (ch_destqport conf p))
+      state_inv Map.empty (recv_sim_mid2 k (ch_destqport conf p)) (recv_sim_mid1 k (ch_destqport conf p))
+      None
+      recv\<^sub>a_rely recv\<^sub>a_guar"
+  apply auto
+  apply (rule If_Comm_Branch_Sound)
+        apply simp+
+      apply (simp add: Stable_def related_transitions_def)
+       apply auto
+   apply (rule_tac \<zeta>\<^sub>1 = Map.empty and \<gamma>\<^sub>1 = "recv_sim_none_if_mid k (ch_destqport conf p)" in Seq_Skip_Sound)
       apply blast
-  apply(simp add: stable_def)+
-   apply(rule rghoare_p.Basic, simp)
-      apply auto[1]
-  apply(simp add: stable_def)+
-  apply(rule rghoare_p.Seq[where mid="{}"])
-   apply(rule rghoare_p.Basic)
-       apply(simp add:stable_def)+
-  apply(rule rghoare_p.Basic, simp)
-     apply(simp add:stable_def)+
-  done
-
-lemma Recv_Que_sat_SCE: "sc_p_sat (the (body_e (Recv_Que_Message k p))) (Recv_Que_Message k p )"
-  apply (simp add: body_def Recv_Que_Message_def)
-  apply (rule_tac pre = "\<lbrace>is_dest_qport conf p \<and> (\<exists>y. \<acute>cur (c2s conf k) = Some y) \<and> port_of_part conf p (the (\<acute>cur (c2s conf k)))\<rbrace>" 
-          and rely = Id and post = "\<lbrace>True\<rbrace>" and guar = "\<lbrace>\<ordfeminine>cur = \<ordmasculine>cur \<and> \<ordfeminine>partst = \<ordmasculine>partst \<and> 
-          ((is_dest_qport conf p \<and> \<ordmasculine>cur ((c2s conf) k) \<noteq> None \<and> port_of_part conf p (the (\<ordmasculine>cur ((c2s conf) k)))) 
-          \<longrightarrow> (\<forall>c. c \<noteq> ch_destqport conf p \<longrightarrow> \<ordfeminine>qbuf c = \<ordmasculine>qbuf c \<and> \<ordfeminine>qbufsize c = \<ordmasculine>qbufsize c) \<and> 
-          (\<ordmasculine>qbufsize (ch_destqport conf p) > 0 \<longrightarrow> \<ordfeminine>qbufsize (ch_destqport conf p) = \<ordmasculine>qbufsize (ch_destqport conf p) - 1) \<and>
-          (\<ordmasculine>qbufsize (ch_destqport conf p) = 0 \<longrightarrow> \<ordfeminine>qbuf = \<ordmasculine>qbuf \<and> \<ordfeminine>qbufsize  = \<ordmasculine>qbufsize)) 
-          \<and> ((\<not>(is_dest_qport conf p \<and> \<ordmasculine>cur ((c2s conf) k) \<noteq> None \<and> port_of_part conf p (the (\<ordmasculine>cur ((c2s conf) k)))))
-          \<longrightarrow> (\<ordfeminine>qbuf  = \<ordmasculine>qbuf  \<and> \<ordfeminine>qbufsize  = \<ordmasculine>qbufsize))\<rbrace>" in sc_p_sat.Await)
-    apply (rule rghoare_p.Await, simp)
-      apply (simp add: stable_def)+
-    apply (rule allI)
-  using Recv_Que_sat_SCE_h1 apply auto[1]
+     apply simp
+    apply (rule Basic_None_Sound)
+         apply blast+
+       apply (simp add: Stable_def related_transitions_def)
+       apply fastforce
+      apply (simp add: Stable_def related_transitions_def)
+      apply fastforce
+     apply (simp add: state_inv_def)
+     apply auto[1]
+    apply simp
+   apply (rule Basic_None_Sound)
+        apply blast+
+      apply (simp add: Stable_def related_transitions_def)
+      apply fastforce
+     apply (simp add: Stable_def related_transitions_def)
+     apply fastforce
+    apply (simp add: state_inv_def)
+    apply auto[1]
    apply simp
-  apply (simp add: domevt_def get_evt_core_def Recv_Que_Message_def label_def get_evt_el_def get_evt_label_def, clarify)
-  apply (case_tac u)
-    apply (simp add: state_equiv_def state_obs_part_def)
-    apply (rule s0_update_help)
-     apply (smt (z3) State.ext_inject State.surjective State.update_convs(3) State.update_convs(4))
-    apply (rule obs_cap_equiv, clarsimp)
-  apply (subgoal_tac "qbufsize s1 c = qbufsize s2 c")
-     apply (metis bot_nat_0.not_eq_extremum)
-    apply (metis (no_types, lifting) State.ext_inject State.surjective State.update_convs(3) obs_cap_part_def)
-   apply (simp add: state_equiv_def state_obs_sched_def)
-  using state_equiv_def state_obs.simps(3) by presburger
+  apply (simp add: Skip_def, rule Basic_None_Sound)
+       apply blast+
+     apply (simp add: Stable_def related_transitions_def)
+     apply fastforce
+    apply (simp add: Stable_def related_transitions_def)
+    apply fastforce
+   apply (simp add: state_inv_def)
+  by auto
 
-lemma uwce_SCE_help: "\<forall>k. ef \<in> all_evts_es (fst (ARINCXKernel_Spec k)) \<longrightarrow> sc_p \<Gamma> (the (body_e (E\<^sub>e ef))) (E\<^sub>e ef)"
-  proof -
-  {
-    fix k
-    assume p0: "ef\<in>all_evts_es (fst (ARINCXKernel_Spec k))" 
-    then have "ef\<in>all_evts_es (fst (EvtSys_on_Core_RGF k))" by (simp add:ARINCXKernel_Spec_def)
-    then have "ef\<in>insert (Core_Init_RGF k) (all_evts_es (fst (EvtSys1_on_Core_RGF k)))" 
-      by (simp add:EvtSys_on_Core_RGF_def)
-    then have "ef = (Core_Init_RGF k) \<or> ef\<in>all_evts_es (fst (EvtSys1_on_Core_RGF k))" by auto
-    then have "sc_p \<Gamma> (the (body_e (E\<^sub>e ef))) (E\<^sub>e ef)"
-      proof
-        assume a0: "ef = Core_Init_RGF k"
-        then show ?thesis
-          by (simp add: Core_Init_RGF_def Core_Init_sat_SCE E\<^sub>e_def sc_p_sound)
-      next
-        assume a1: "ef\<in>all_evts_es (fst (EvtSys1_on_Core_RGF k))"
-        then have "ef\<in>{ef. \<exists>p. ef = Schedule_RGF k p} \<union>
-                      {ef. \<exists>p m. ef = Send_Que_Message_RGF k p m} \<union>
-                      {ef. \<exists>p. ef = Recv_Que_Message_RGF k p}" 
-          using all_evts_es_esys EvtSys1_on_Core_RGF_def by auto
-        then have "ef\<in>{ef. \<exists>p. ef = Schedule_RGF k p} 
-                  \<or> ef\<in>{ef. \<exists>p m. ef = Send_Que_Message_RGF k p m} 
-                  \<or> ef\<in>{ef. \<exists>p. ef = Recv_Que_Message_RGF k p}" by auto
-        then show ?thesis
-          proof
-            assume "ef\<in>{ef. \<exists>p. ef = Schedule_RGF k p}"
-            then have "\<exists>p. ef = Schedule_RGF k p" by auto
-            then obtain p where "ef = Schedule_RGF k p" by auto
-            then show ?thesis 
-              by (simp add: E\<^sub>e_def Schedule_RGF_def Schedule_sat_SCE sc_p_sound)
-          next
-            assume "ef\<in>{ef. \<exists>p m. ef = Send_Que_Message_RGF k p m}
-                    \<or> ef\<in>{ef. \<exists>p. ef = Recv_Que_Message_RGF k p}"
-            then show ?thesis 
-              proof
-                assume "ef\<in>{ef. \<exists>p m. ef = Send_Que_Message_RGF k p m}"
-                then have "\<exists>p m. ef = Send_Que_Message_RGF k p m" by auto
-                then obtain p and m where "ef = Send_Que_Message_RGF k p m" by auto
-                then show ?thesis 
-                  by (simp add: E\<^sub>e_def Send_Que_Message_RGF_def Send_Que_sat_SCE sc_p_sound)
-              next
-                assume "ef\<in>{ef. \<exists>p. ef = Recv_Que_Message_RGF k p}"
-                then have "\<exists>p. ef = Recv_Que_Message_RGF k p" by auto
-                then obtain p where "ef = Recv_Que_Message_RGF k p" by auto
-                then show ?thesis 
-                  by (simp add: E\<^sub>e_def Recv_Que_Message_RGF_def Recv_Que_sat_SCE sc_p_sound)
-              qed
-          qed
-      qed
-  }
-  then show ?thesis by auto
-qed
+lemma recv_sim: "prog_sim_pre (Some 
+      (AWAIT \<acute>qlock\<^sub>c (ch_destqport conf p) = None THEN
+        \<acute>qlock\<^sub>c := \<acute>qlock\<^sub>c (ch_destqport conf p := Some k)
+      END;;
+      IF \<acute>qbufsize\<^sub>c (ch_destqport conf p) > 0 THEN 
+        \<acute>qbuf\<^sub>c := \<acute>qbuf\<^sub>c (ch_destqport conf p := tl (\<acute>qbuf\<^sub>c (ch_destqport conf p)));;
+        \<acute>qbufsize\<^sub>c := \<acute>qbufsize\<^sub>c (ch_destqport conf p := \<acute>qbufsize\<^sub>c (ch_destqport conf p) - 1)
+      FI;;
+      ATOMIC
+        \<acute>qlock\<^sub>c := \<acute>qlock\<^sub>c (ch_destqport conf p := None);;
+        \<acute>obsize\<^sub>c := \<acute>obsize\<^sub>c (ch_destqport conf p := \<acute>qbufsize\<^sub>c (ch_destqport conf p))
+      END))
+      (recv\<^sub>c_rely k (ch_destqport conf p)) (recv\<^sub>c_guar k (ch_destqport conf p)) 
+      state_inv (recv_map k p) recv_pre recv_post
+      (Some 
+      (ATOMIC
+         IF \<acute>qbufsize\<^sub>a (ch_destqport conf p) > 0 THEN 
+           \<acute>qbuf\<^sub>a := \<acute>qbuf\<^sub>a (ch_destqport conf p := tl (\<acute>qbuf\<^sub>a (ch_destqport conf p)));;
+           \<acute>qbufsize\<^sub>a := \<acute>qbufsize\<^sub>a (ch_destqport conf p := \<acute>qbufsize\<^sub>a (ch_destqport conf p) - 1)
+         FI
+      END))
+      recv\<^sub>a_rely recv\<^sub>a_guar"
+  apply (rule_tac \<zeta>\<^sub>1 = Map.empty and \<gamma>\<^sub>1 = "recv_sim_mid1 k (ch_destqport conf p)" in Seq_Skip_Sound)
+     apply (simp add: recv_map_def)+
+   apply (rule_tac \<zeta>\<^sub>1 = Map.empty and \<gamma>\<^sub>1 = "recv_sim_mid2 k (ch_destqport conf p)" in Seq_Skip_Sound)
+      apply simp+
+  using recv_sim_none1 apply auto[1]
+  using recv_sim_none2 apply auto[1]
+  using recv_unlock_sim by auto
 
-interpretation PiCore_IFS.InfoFlow ptranI petranI None \<Gamma> C0 "exec_step \<Gamma>" interf state_equiv state_obs domevt
-proof
-  show "\<forall>a b c u. a \<sim>u\<sim> b \<and> b \<sim>u\<sim> c \<longrightarrow> a \<sim>u\<sim> c"
-    using state_equiv_def by presburger
-  show "\<forall>a b u. a \<sim>u\<sim> b \<longrightarrow> b \<sim>u\<sim> a"
-    using simp_vpeq_sym by blast
-  show "\<forall>a u. a \<sim>u\<sim> a"
-    by (simp add: simp_vpeq_refl)
-  show "\<And>a. exec_step \<Gamma> a \<equiv> {(P, Q). \<Gamma> \<turnstile> P -pes-actk a\<rightarrow> Q \<and>
-       ((\<exists>e k. actk a = EvtEnt e\<sharp>k \<and> eventof a = e \<and> domevt (gets P) e = domain a) \<or>
-       (\<exists>c k. actk a = Cmd c\<sharp>k \<and> eventof a = getx P k \<and> domevt (gets P) (eventof a) = domain a))}"
-    by (simp add: exec_step_def)
-qed
+      
 
-lemma uwc_oc: "observed_consistentC"
-  apply(simp add:observed_consistentC_def)
-  by(simp add:state_equiv_def)
-
-lemma uwc_lr: "InfoFlow.local_respectC C0 (exec_step \<Gamma>) interf state_equiv"
-  apply (rule rg_lr_imp_lr)
-  apply (simp add: local_respect_events_def all_evts_def, clarify)
-  using all_evts_def[of ARINCXKernel_Spec] uwce_LRE_help 
-  using noninterf_def  by blast
-
-lemma uwc_sc: "InfoFlow.weak_step_consistentC C0 (exec_step \<Gamma>) interf state_equiv"
-  apply (rule rg_sc_imp_sc)
-  apply (simp add: step_consistent_events_def all_evts_def, clarify)
-  using all_evts_def[of ARINCXKernel_Spec] uwce_SCE_help
-  using noninterf_def by metis
-
-lemma "SM_IFS.nonleakage C0 (exec_step \<Gamma>) domain obsC vpeqC interf"
-  by (simp add: PiCore_nonleakage uwc_oc uwc_sc)
-
-theorem "SM_IFS.noninfluence0 C0 (exec_step \<Gamma>) domain obsC vpeqC interf"
-  by (simp add: PiCore_noninfluence0 uwc_lr uwc_oc uwc_sc)
 
 end
